<?xml version="1.0"?>
<rdf:RDF xmlns="http://semantic-web-kms.edu.et/wdo/"
     xml:base="http://semantic-web-kms.edu.et/wdo/"
     xmlns:dc="http://purl.org/dc/elements/1.1/"
     xmlns:bfo="http://purl.obolibrary.org/obo/"
     xmlns:owl="http://www.w3.org/2002/07/owl#"
     xmlns:rdf="http://www.w3.org/1999/02/22-rdf-syntax-ns#"
     xmlns:wdo="http://semantic-web-kms.edu.et/wdo#"
     xmlns:xml="http://www.w3.org/XML/1998/namespace"
     xmlns:xsd="http://www.w3.org/2001/XMLSchema#"
     xmlns:rdfs="http://www.w3.org/2000/01/rdf-schema#"
     xmlns:skos="http://www.w3.org/2004/02/skos/core#"
     xmlns:terms="http://purl.org/dc/terms/">
    <owl:Ontology rdf:about="http://semantic-web-kms.edu.et/wdo/">
        <owl:versionIRI rdf:resource="http://semantic-web-kms.edu.et/wdo/1.0.0"/>
        <owl:imports rdf:resource="http://purl.obolibrary.org/obo/bfo/2020/bfo-core.owl"/>
        <dc:creator xml:lang="en">Group One, CoSc 6232 (Spring 2025)</dc:creator>
        <dc:description xml:lang="en">An ontology designed to support semantic-based explicit knowledge management for web development projects. WDO provides a structured vocabulary for representing artifacts extracted from local repositories, including codebase components (classes, functions, attributes), documentation, licensing information, READMEs, best practices, and various digital assets. Its goal is to facilitate the organization, retrieval, and understanding of explicit knowledge within web development lifecycles.</dc:description>
        <dc:identifier>WDO</dc:identifier>
        <dc:publisher xml:lang="en">Department of Computer Science, Addis Ababa University</dc:publisher>
        <dc:rights xml:lang="en">This ontology is made available under the Creative Commons Attribution 4.0 International (CC BY 4.0) license.</dc:rights>
        <dc:title xml:lang="en">Web Development Ontology (WDO) for Knowledge Management</dc:title>
        <rdfs:comment xml:lang="en">Web Development Ontology (WDO) is aligned with Basic Formal Ontology (BFO) 2020 (http://purl.obolibrary.org/obo/bfo/2020/bfo-core.owl) as its top-level ontology and incorporates and adapts concepts from ontologies like DoCO and CodeOntology where relevant to the web development domain. This version has been extended to include more specific types of file carriers and content entities, and has been refined for greater formal correctness.</rdfs:comment>
        <rdfs:seeAlso rdf:resource="https://github.com/shama-llama/semantic-web-kms"/>
        <owl:versionInfo xml:lang="en">Version 1.0.0 - First fully working version.</owl:versionInfo>
    </owl:Ontology>
    


    <!-- 
    ///////////////////////////////////////////////////////////////////////////////////////
    //
    // Annotation properties
    //
    ///////////////////////////////////////////////////////////////////////////////////////
     -->

    


    <!-- http://purl.org/dc/elements/1.1/creator -->

    <owl:AnnotationProperty rdf:about="http://purl.org/dc/elements/1.1/creator"/>
    


    <!-- http://purl.org/dc/elements/1.1/description -->

    <owl:AnnotationProperty rdf:about="http://purl.org/dc/elements/1.1/description"/>
    


    <!-- http://purl.org/dc/elements/1.1/publisher -->

    <owl:AnnotationProperty rdf:about="http://purl.org/dc/elements/1.1/publisher"/>
    


    <!-- http://purl.org/dc/elements/1.1/rights -->

    <owl:AnnotationProperty rdf:about="http://purl.org/dc/elements/1.1/rights"/>
    


    <!-- http://purl.org/dc/elements/1.1/title -->

    <owl:AnnotationProperty rdf:about="http://purl.org/dc/elements/1.1/title"/>
    


    <!-- http://purl.org/dc/terms/creator -->

    <owl:AnnotationProperty rdf:about="http://purl.org/dc/terms/creator"/>
    


    <!-- http://purl.org/dc/terms/description -->

    <owl:AnnotationProperty rdf:about="http://purl.org/dc/terms/description"/>
    


    <!-- http://purl.org/dc/terms/identifier -->

    <owl:AnnotationProperty rdf:about="http://purl.org/dc/terms/identifier"/>
    


    <!-- http://purl.org/dc/terms/publisher -->

    <owl:AnnotationProperty rdf:about="http://purl.org/dc/terms/publisher"/>
    


    <!-- http://purl.org/dc/terms/rights -->

    <owl:AnnotationProperty rdf:about="http://purl.org/dc/terms/rights"/>
    


    <!-- http://purl.org/dc/terms/title -->

    <owl:AnnotationProperty rdf:about="http://purl.org/dc/terms/title"/>
    


    <!-- http://semantic-web-kms.edu.et/wdo#fileExtension -->

    <owl:AnnotationProperty rdf:about="http://semantic-web-kms.edu.et/wdo#fileExtension">
        <rdfs:label xml:lang="en">file extension</rdfs:label>
        <skos:definition xml:lang="en">An annotation property to specify the file extension of a Digital Information Carrier (e.g., &apos;java&apos;, &apos;py&apos;, &apos;md&apos;, &apos;png&apos;).</skos:definition>
        <rdfs:range rdf:resource="http://www.w3.org/2001/XMLSchema#string"/>
    </owl:AnnotationProperty>
    


    <!-- http://semantic-web-kms.edu.et/wdo#programmingLanguage -->

    <owl:AnnotationProperty rdf:about="http://semantic-web-kms.edu.et/wdo#programmingLanguage">
        <rdfs:label xml:lang="en">programming language</rdfs:label>
        <skos:definition xml:lang="en">An annotation property to specify the programming language of a software code component or file.</skos:definition>
        <rdfs:range rdf:resource="http://www.w3.org/2001/XMLSchema#string"/>
    </owl:AnnotationProperty>
    


    <!-- http://semantic-web-kms.edu.et/wdo#sourceRepositoryURL -->

    <owl:AnnotationProperty rdf:about="http://semantic-web-kms.edu.et/wdo#sourceRepositoryURL">
        <rdfs:label xml:lang="en">source repository URL</rdfs:label>
        <skos:definition xml:lang="en">An annotation property to specify the URL or path of the local repository from which an artifact was extracted.</skos:definition>
        <rdfs:range rdf:resource="http://www.w3.org/2001/XMLSchema#anyURI"/>
    </owl:AnnotationProperty>
    


    <!-- http://www.w3.org/2000/01/rdf-schema#comment -->

    <owl:AnnotationProperty rdf:about="http://www.w3.org/2000/01/rdf-schema#comment"/>
    


    <!-- http://www.w3.org/2000/01/rdf-schema#seeAlso -->

    <owl:AnnotationProperty rdf:about="http://www.w3.org/2000/01/rdf-schema#seeAlso"/>
    


    <!-- http://www.w3.org/2002/07/owl#versionInfo -->

    <owl:AnnotationProperty rdf:about="http://www.w3.org/2002/07/owl#versionInfo"/>
    


    <!-- http://www.w3.org/2004/02/skos/core#definition -->

    <owl:AnnotationProperty rdf:about="http://www.w3.org/2004/02/skos/core#definition"/>
    


    <!-- http://www.w3.org/2004/02/skos/core#example -->

    <owl:AnnotationProperty rdf:about="http://www.w3.org/2004/02/skos/core#example"/>
    


    <!-- 
    ///////////////////////////////////////////////////////////////////////////////////////
    //
    // Datatypes
    //
    ///////////////////////////////////////////////////////////////////////////////////////
     -->

    


    <!-- http://www.w3.org/2001/XMLSchema#duration -->

    <rdfs:Datatype rdf:about="http://www.w3.org/2001/XMLSchema#duration"/>
    


    <!-- 
    ///////////////////////////////////////////////////////////////////////////////////////
    //
    // Object Properties
    //
    ///////////////////////////////////////////////////////////////////////////////////////
     -->

    


    <!-- http://semantic-web-kms.edu.et/wdo#accesses -->

    <owl:ObjectProperty rdf:about="http://semantic-web-kms.edu.et/wdo#accesses">
        <rdfs:domain rdf:resource="http://semantic-web-kms.edu.et/wdo#FunctionDefinition"/>
        <rdfs:range rdf:resource="http://semantic-web-kms.edu.et/wdo#AttributeDeclaration"/>
        <dc:identifier>WDO_OP:0000021</dc:identifier>
        <rdfs:label xml:lang="en">accesses</rdfs:label>
        <skos:definition xml:lang="en">A relation indicating that a function or method reads from or writes to a variable, attribute, or field.</skos:definition>
    </owl:ObjectProperty>
    


    <!-- http://semantic-web-kms.edu.et/wdo#bearerOfInformation -->

    <owl:ObjectProperty rdf:about="http://semantic-web-kms.edu.et/wdo#bearerOfInformation">
        <owl:inverseOf rdf:resource="http://semantic-web-kms.edu.et/wdo#informationBorneBy"/>
        <rdfs:domain rdf:resource="http://semantic-web-kms.edu.et/wdo#DigitalInformationCarrier"/>
        <rdfs:range rdf:resource="http://semantic-web-kms.edu.et/wdo#InformationContentEntity"/>
        <dc:identifier>WDO_OP:0000001</dc:identifier>
        <rdfs:label xml:lang="en">bearer of information</rdfs:label>
        <skos:definition xml:lang="en">A relation between a Digital Information Carrier (e.g., a file) and the InformationContentEntity it encodes or represents.</skos:definition>
    </owl:ObjectProperty>
    


    <!-- http://semantic-web-kms.edu.et/wdo#callsFunction -->

    <owl:ObjectProperty rdf:about="http://semantic-web-kms.edu.et/wdo#callsFunction">
        <rdfs:domain rdf:resource="http://semantic-web-kms.edu.et/wdo#FunctionCallSite"/>
        <rdfs:range rdf:resource="http://semantic-web-kms.edu.et/wdo#FunctionDefinition"/>
        <dc:identifier>WDO_OP:0000033</dc:identifier>
        <rdfs:label xml:lang="en">calls function</rdfs:label>
        <skos:definition xml:lang="en">A relation between a FunctionCallSite and the FunctionDefinition it invokes.</skos:definition>
    </owl:ObjectProperty>
    


    <!-- http://semantic-web-kms.edu.et/wdo#compiles -->

    <owl:ObjectProperty rdf:about="http://semantic-web-kms.edu.et/wdo#compiles">
        <rdfs:domain rdf:resource="http://semantic-web-kms.edu.et/wdo#BuildScript"/>
        <rdfs:range rdf:resource="http://semantic-web-kms.edu.et/wdo#SourceCodeFile"/>
        <rdfs:label xml:lang="en">compiles</rdfs:label>
        <skos:definition xml:lang="en">A relation from a build script to the source code files it processes during compilation.</skos:definition>
    </owl:ObjectProperty>
    


    <!-- http://semantic-web-kms.edu.et/wdo#conformsToGuideline -->

    <owl:ObjectProperty rdf:about="http://semantic-web-kms.edu.et/wdo#conformsToGuideline">
        <rdfs:domain rdf:resource="http://purl.obolibrary.org/obo/BFO_0000001"/>
        <rdfs:range rdf:resource="http://semantic-web-kms.edu.et/wdo#BestPracticeGuideline"/>
        <dc:identifier>WDO_OP:0000006</dc:identifier>
        <rdfs:label xml:lang="en">conforms to guideline</rdfs:label>
        <skos:definition xml:lang="en">A relation indicating that an entity (e.g., SoftwareCode, a process) adheres to a BestPracticeGuideline.</skos:definition>
    </owl:ObjectProperty>
    


    <!-- http://semantic-web-kms.edu.et/wdo#copiesFrom -->

    <owl:ObjectProperty rdf:about="http://semantic-web-kms.edu.et/wdo#copiesFrom">
        <rdfs:domain rdf:resource="http://semantic-web-kms.edu.et/wdo#DockerfileSpecification"/>
        <rdfs:range rdf:resource="http://semantic-web-kms.edu.et/wdo#DigitalInformationCarrier"/>
        <rdfs:label xml:lang="en">copies from</rdfs:label>
        <skos:definition xml:lang="en">A relation indicating a Dockerfile copies a specific file into the container image.</skos:definition>
    </owl:ObjectProperty>
    


    <!-- http://semantic-web-kms.edu.et/wdo#declaresCode -->

    <owl:ObjectProperty rdf:about="http://semantic-web-kms.edu.et/wdo#declaresCode">
        <rdfs:subPropertyOf rdf:resource="http://purl.obolibrary.org/obo/BFO_0000178"/>
        <rdfs:domain rdf:resource="http://semantic-web-kms.edu.et/wdo#SoftwareCode"/>
        <rdfs:range rdf:resource="http://semantic-web-kms.edu.et/wdo#SoftwareCode"/>
        <dc:identifier>WDO_OP:0000007</dc:identifier>
        <rdfs:label xml:lang="en">declares code</rdfs:label>
        <skos:definition xml:lang="en">A relation between a SoftwareCode entity (like a Class or Package) and another SoftwareCode it declares (like a Method, Field, or inner Class).</skos:definition>
    </owl:ObjectProperty>
    


    <!-- http://semantic-web-kms.edu.et/wdo#declaresVariable -->

    <owl:ObjectProperty rdf:about="http://semantic-web-kms.edu.et/wdo#declaresVariable">
        <rdfs:domain rdf:resource="http://semantic-web-kms.edu.et/wdo#FunctionDefinition"/>
        <rdfs:range rdf:resource="http://semantic-web-kms.edu.et/wdo#VariableDeclaration"/>
        <rdfs:label xml:lang="en">declares variable</rdfs:label>
        <skos:definition xml:lang="en">A relation between a function and a variable declaration within its local scope.</skos:definition>
    </owl:ObjectProperty>
    


    <!-- http://semantic-web-kms.edu.et/wdo#documentsEntity -->

    <owl:ObjectProperty rdf:about="http://semantic-web-kms.edu.et/wdo#documentsEntity">
        <owl:inverseOf rdf:resource="http://semantic-web-kms.edu.et/wdo#isDocumentedBy"/>
        <rdfs:domain rdf:resource="http://semantic-web-kms.edu.et/wdo#Documentation"/>
        <rdfs:range rdf:resource="http://purl.obolibrary.org/obo/BFO_0000001"/>
        <dc:identifier>WDO_OP:0000004</dc:identifier>
        <rdfs:label xml:lang="en">documents entity</rdfs:label>
        <skos:definition xml:lang="en">A relation between a Documentation entity and the entity (e.g., SoftwareCode, WebDevelopmentProject) it describes or explains.</skos:definition>
    </owl:ObjectProperty>
    


    <!-- http://semantic-web-kms.edu.et/wdo#embedsCode -->

    <owl:ObjectProperty rdf:about="http://semantic-web-kms.edu.et/wdo#embedsCode">
        <rdfs:subPropertyOf rdf:resource="http://purl.obolibrary.org/obo/BFO_0000178"/>
        <rdfs:domain rdf:resource="http://semantic-web-kms.edu.et/wdo#Template"/>
        <rdfs:range rdf:resource="http://semantic-web-kms.edu.et/wdo#SoftwareCode"/>
        <dc:identifier>WDO_OP:0000024</dc:identifier>
        <rdfs:label xml:lang="en">embeds code</rdfs:label>
        <skos:definition xml:lang="en">A relation indicating that a template contains embedded software code that is processed at runtime.</skos:definition>
    </owl:ObjectProperty>
    


    <!-- http://semantic-web-kms.edu.et/wdo#extendsType -->

    <owl:ObjectProperty rdf:about="http://semantic-web-kms.edu.et/wdo#extendsType">
        <rdfs:domain rdf:resource="http://semantic-web-kms.edu.et/wdo#ComplexType"/>
        <rdfs:range rdf:resource="http://semantic-web-kms.edu.et/wdo#ComplexType"/>
        <dc:identifier>WDO_OP:0000010</dc:identifier>
        <rdfs:label xml:lang="en">extends type</rdfs:label>
        <skos:definition xml:lang="en">A relation indicating that a ComplexType (e.g. a class) extends another ComplexType (e.g. a superclass or interface).</skos:definition>
    </owl:ObjectProperty>
    


    <!-- http://semantic-web-kms.edu.et/wdo#generates -->

    <owl:ObjectProperty rdf:about="http://semantic-web-kms.edu.et/wdo#generates">
        <rdfs:domain rdf:resource="http://semantic-web-kms.edu.et/wdo#SoftwareCode"/>
        <rdfs:range rdf:resource="http://semantic-web-kms.edu.et/wdo#InformationContentEntity"/>
        <rdfs:label xml:lang="en">generates</rdfs:label>
        <skos:definition xml:lang="en">A relation for code generation, where one piece of code produces another.</skos:definition>
    </owl:ObjectProperty>
    


    <!-- http://semantic-web-kms.edu.et/wdo#hasArgument -->

    <owl:ObjectProperty rdf:about="http://semantic-web-kms.edu.et/wdo#hasArgument">
        <rdfs:domain rdf:resource="http://semantic-web-kms.edu.et/wdo#FunctionCallSite"/>
        <rdfs:range rdf:resource="http://semantic-web-kms.edu.et/wdo#SoftwareCode"/>
        <dc:identifier>WDO_OP:0000034</dc:identifier>
        <rdfs:label xml:lang="en">has argument</rdfs:label>
        <skos:definition xml:lang="en">A relation between a FunctionCallSite and a SoftwareCode entity (such as a VariableDeclaration or a literal value) passed as an argument.</skos:definition>
    </owl:ObjectProperty>
    


    <!-- http://semantic-web-kms.edu.et/wdo#hasCommit -->

    <owl:ObjectProperty rdf:about="http://semantic-web-kms.edu.et/wdo#hasCommit">
        <rdfs:domain rdf:resource="http://semantic-web-kms.edu.et/wdo#Repository"/>
        <rdfs:range rdf:resource="http://semantic-web-kms.edu.et/wdo#Commit"/>
        <rdfs:label xml:lang="en">has commit</rdfs:label>
        <skos:definition xml:lang="en">A relation linking a repository to the commits in its history.</skos:definition>
    </owl:ObjectProperty>
    


    <!-- http://semantic-web-kms.edu.et/wdo#hasDocumentComponent -->

    <owl:ObjectProperty rdf:about="http://semantic-web-kms.edu.et/wdo#hasDocumentComponent">
        <rdfs:subPropertyOf rdf:resource="http://purl.obolibrary.org/obo/BFO_0000178"/>
        <rdf:type rdf:resource="http://www.w3.org/2002/07/owl#TransitiveProperty"/>
        <rdfs:domain rdf:resource="http://semantic-web-kms.edu.et/wdo#InformationContentEntity"/>
        <rdfs:range rdf:resource="http://semantic-web-kms.edu.et/wdo#InformationContentEntity"/>
        <dc:identifier>WDO_OP:0000015</dc:identifier>
        <rdfs:label xml:lang="en">has document component</rdfs:label>
        <skos:definition xml:lang="en">A relation between an InformationContentEntity (like a document or section) and a smaller InformationContentEntity that is one of its components (like a paragraph or list).</skos:definition>
    </owl:ObjectProperty>
    


    <!-- http://semantic-web-kms.edu.et/wdo#hasField -->

    <owl:ObjectProperty rdf:about="http://semantic-web-kms.edu.et/wdo#hasField">
        <rdfs:subPropertyOf rdf:resource="http://semantic-web-kms.edu.et/wdo#declaresCode"/>
        <rdfs:domain rdf:resource="http://semantic-web-kms.edu.et/wdo#ComplexType"/>
        <rdfs:range rdf:resource="http://semantic-web-kms.edu.et/wdo#AttributeDeclaration"/>
        <dc:identifier>WDO_OP:0000009</dc:identifier>
        <rdfs:label xml:lang="en">has field</rdfs:label>
        <skos:definition xml:lang="en">A relation between a ComplexType and an AttributeDeclaration that it declares as a field.</skos:definition>
    </owl:ObjectProperty>
    


    <!-- http://semantic-web-kms.edu.et/wdo#hasMethod -->

    <owl:ObjectProperty rdf:about="http://semantic-web-kms.edu.et/wdo#hasMethod">
        <rdfs:subPropertyOf rdf:resource="http://semantic-web-kms.edu.et/wdo#declaresCode"/>
        <owl:inverseOf rdf:resource="http://semantic-web-kms.edu.et/wdo#isMethodOf"/>
        <rdfs:domain rdf:resource="http://semantic-web-kms.edu.et/wdo#ComplexType"/>
        <rdfs:range rdf:resource="http://semantic-web-kms.edu.et/wdo#FunctionDefinition"/>
        <dc:identifier>WDO_OP:0000008</dc:identifier>
        <rdfs:label xml:lang="en">has method</rdfs:label>
        <skos:definition xml:lang="en">A relation between a ClassDefinition or InterfaceDefinition and a FunctionDefinition that it declares as a method.</skos:definition>
    </owl:ObjectProperty>
    


    <!-- http://semantic-web-kms.edu.et/wdo#hasParameter -->

    <owl:ObjectProperty rdf:about="http://semantic-web-kms.edu.et/wdo#hasParameter">
        <rdfs:subPropertyOf rdf:resource="http://semantic-web-kms.edu.et/wdo#declaresCode"/>
        <rdfs:domain rdf:resource="http://semantic-web-kms.edu.et/wdo#FunctionDefinition"/>
        <rdfs:range rdf:resource="http://semantic-web-kms.edu.et/wdo#Parameter"/>
        <dc:identifier>WDO_OP:0000012</dc:identifier>
        <rdfs:label xml:lang="en">has parameter</rdfs:label>
        <skos:definition xml:lang="en">A relation between a FunctionDefinition and a Parameter that it declares.</skos:definition>
    </owl:ObjectProperty>
    


    <!-- http://semantic-web-kms.edu.et/wdo#hasProjectOutput -->

    <owl:ObjectProperty rdf:about="http://semantic-web-kms.edu.et/wdo#hasProjectOutput">
        <rdfs:subPropertyOf rdf:resource="http://purl.obolibrary.org/obo/BFO_0000057"/>
        <rdfs:domain rdf:resource="http://semantic-web-kms.edu.et/wdo#WebDevelopmentProject"/>
        <rdfs:range rdf:resource="http://semantic-web-kms.edu.et/wdo#InformationContentEntity"/>
        <dc:identifier>WDO_OP:0000005</dc:identifier>
        <rdfs:label xml:lang="en">has project output</rdfs:label>
        <skos:definition xml:lang="en">A relation between a WebDevelopmentProject (a process) and an InformationContentEntity that is its output.</skos:definition>
    </owl:ObjectProperty>
    


    <!-- http://semantic-web-kms.edu.et/wdo#hasRepository -->

    <owl:ObjectProperty rdf:about="http://semantic-web-kms.edu.et/wdo#hasRepository">
        <rdfs:domain rdf:resource="http://semantic-web-kms.edu.et/wdo#WebDevelopmentProject"/>
        <rdfs:range rdf:resource="http://semantic-web-kms.edu.et/wdo#Repository"/>
        <rdfs:label xml:lang="en">has repository</rdfs:label>
        <skos:definition xml:lang="en">Links a project to its source code repository.</skos:definition>
    </owl:ObjectProperty>
    


    <!-- http://semantic-web-kms.edu.et/wdo#hasResource -->

    <owl:ObjectProperty rdf:about="http://semantic-web-kms.edu.et/wdo#hasResource">
        <rdfs:range rdf:resource="http://semantic-web-kms.edu.et/wdo#DigitalInformationCarrier"/>
        <dc:identifier>WDO_OP:0000035</dc:identifier>
        <rdfs:label xml:lang="en">has resource</rdfs:label>
        <skos:definition xml:lang="en">A relation linking a project to a digital information carrier (file or asset) that is part of the project.</skos:definition>
    </owl:ObjectProperty>
    


    <!-- http://semantic-web-kms.edu.et/wdo#hasReturnType -->

    <owl:ObjectProperty rdf:about="http://semantic-web-kms.edu.et/wdo#hasReturnType">
        <rdfs:domain rdf:resource="http://semantic-web-kms.edu.et/wdo#FunctionDefinition"/>
        <rdfs:range rdf:resource="http://semantic-web-kms.edu.et/wdo#Type"/>
        <dc:identifier>WDO_OP:0000013</dc:identifier>
        <rdfs:label xml:lang="en">has return type</rdfs:label>
        <skos:definition xml:lang="en">A relation specifying the Type that a FunctionDefinition returns.</skos:definition>
    </owl:ObjectProperty>
    


    <!-- http://semantic-web-kms.edu.et/wdo#hasSoftwareLicense -->

    <owl:ObjectProperty rdf:about="http://semantic-web-kms.edu.et/wdo#hasSoftwareLicense">
        <rdfs:domain rdf:resource="http://semantic-web-kms.edu.et/wdo#WebDevelopmentProject"/>
        <rdfs:range rdf:resource="http://semantic-web-kms.edu.et/wdo#License"/>
        <dc:identifier>WDO_OP:0000003</dc:identifier>
        <rdfs:label xml:lang="en">has software license</rdfs:label>
        <skos:definition xml:lang="en">A relation between a WebDevelopmentProject and its associated License.</skos:definition>
    </owl:ObjectProperty>
    


    <!-- http://semantic-web-kms.edu.et/wdo#hasSpecificLicense -->

    <owl:ObjectProperty rdf:about="http://semantic-web-kms.edu.et/wdo#hasSpecificLicense">
        <rdfs:domain rdf:resource="http://semantic-web-kms.edu.et/wdo#SoftwareCode"/>
        <rdfs:range rdf:resource="http://semantic-web-kms.edu.et/wdo#License"/>
        <rdfs:label xml:lang="en">has specific license</rdfs:label>
        <skos:definition xml:lang="en">A specific license for a piece of code, potentially overriding the project license.</skos:definition>
    </owl:ObjectProperty>
    


    <!-- http://semantic-web-kms.edu.et/wdo#hasType -->

    <owl:ObjectProperty rdf:about="http://semantic-web-kms.edu.et/wdo#hasType">
        <rdfs:domain rdf:resource="http://semantic-web-kms.edu.et/wdo#SoftwareCode"/>
        <rdfs:range rdf:resource="http://semantic-web-kms.edu.et/wdo#Type"/>
        <dc:identifier>WDO_OP:0000014</dc:identifier>
        <rdfs:label xml:lang="en">has type</rdfs:label>
        <skos:definition xml:lang="en">A relation specifying the Type of a typed SoftwareCode entity (e.g., an attribute, a parameter).</skos:definition>
    </owl:ObjectProperty>
    


    <!-- http://semantic-web-kms.edu.et/wdo#implementsInterface -->

    <owl:ObjectProperty rdf:about="http://semantic-web-kms.edu.et/wdo#implementsInterface">
        <rdfs:domain rdf:resource="http://semantic-web-kms.edu.et/wdo#ClassDefinition"/>
        <rdfs:range rdf:resource="http://semantic-web-kms.edu.et/wdo#InterfaceDefinition"/>
        <dc:identifier>WDO_OP:0000011</dc:identifier>
        <rdfs:label xml:lang="en">implements interface</rdfs:label>
        <skos:definition xml:lang="en">A relation indicating that a ClassDefinition implements an InterfaceDefinition.</skos:definition>
    </owl:ObjectProperty>
    


    <!-- http://semantic-web-kms.edu.et/wdo#imports -->

    <owl:ObjectProperty rdf:about="http://semantic-web-kms.edu.et/wdo#imports">
        <owl:inverseOf rdf:resource="http://semantic-web-kms.edu.et/wdo#isImportedBy"/>
        <rdfs:domain rdf:resource="http://semantic-web-kms.edu.et/wdo#Module"/>
        <rdfs:range rdf:resource="http://semantic-web-kms.edu.et/wdo#Module"/>
        <dc:identifier>WDO_OP:0000028</dc:identifier>
        <rdfs:label xml:lang="en">imports</rdfs:label>
        <skos:definition xml:lang="en">A relation indicating that a module uses or includes another module to access its functionality.</skos:definition>
    </owl:ObjectProperty>
    


    <!-- http://semantic-web-kms.edu.et/wdo#informationBorneBy -->

    <owl:ObjectProperty rdf:about="http://semantic-web-kms.edu.et/wdo#informationBorneBy">
        <rdfs:domain rdf:resource="http://semantic-web-kms.edu.et/wdo#InformationContentEntity"/>
        <rdfs:range rdf:resource="http://semantic-web-kms.edu.et/wdo#DigitalInformationCarrier"/>
        <dc:identifier>WDO_OP:0000002</dc:identifier>
        <rdfs:label xml:lang="en">information borne by</rdfs:label>
        <skos:definition xml:lang="en">A relation between an InformationContentEntity and the Digital Information Carrier (e.g., a file) that encodes it. Inverse of bearerOfInformation.</skos:definition>
    </owl:ObjectProperty>
    


    <!-- http://semantic-web-kms.edu.et/wdo#invokes -->

    <owl:ObjectProperty rdf:about="http://semantic-web-kms.edu.et/wdo#invokes">
        <rdfs:domain rdf:resource="http://semantic-web-kms.edu.et/wdo#FunctionDefinition"/>
        <rdfs:range rdf:resource="http://semantic-web-kms.edu.et/wdo#FunctionDefinition"/>
        <dc:identifier>WDO_OP:0000020</dc:identifier>
        <rdfs:label xml:lang="en">invokes</rdfs:label>
        <skos:definition xml:lang="en">A relation indicating that one function calls another.</skos:definition>
    </owl:ObjectProperty>
    


    <!-- http://semantic-web-kms.edu.et/wdo#isAbout -->

    <owl:ObjectProperty rdf:about="http://semantic-web-kms.edu.et/wdo#isAbout">
        <rdfs:domain rdf:resource="http://semantic-web-kms.edu.et/wdo#InformationContentEntity"/>
        <rdfs:range rdf:resource="http://www.w3.org/2002/07/owl#Thing"/>
        <rdfs:label xml:lang="en">is about</rdfs:label>
        <skos:definition xml:lang="en">A relation indicating that an information content entity (e.g., metadata, description) is about some entity (e.g., a repository, file, or other resource).</skos:definition>
    </owl:ObjectProperty>
    


    <!-- http://semantic-web-kms.edu.et/wdo#isAboutCode -->

    <owl:ObjectProperty rdf:about="http://semantic-web-kms.edu.et/wdo#isAboutCode">
        <rdfs:domain rdf:resource="http://semantic-web-kms.edu.et/wdo#Documentation"/>
        <rdfs:range rdf:resource="http://semantic-web-kms.edu.et/wdo#SoftwareCode"/>
        <dc:identifier>WDO_OP:0000100</dc:identifier>
        <rdfs:label xml:lang="en">is about code</rdfs:label>
        <skos:definition xml:lang="en">A relation indicating that a documentation element, comment, or other resource is specifically about a code entity (e.g., a class, function, or file).</skos:definition>
    </owl:ObjectProperty>
    


    <!-- http://semantic-web-kms.edu.et/wdo#isBasedOn -->

    <owl:ObjectProperty rdf:about="http://semantic-web-kms.edu.et/wdo#isBasedOn">
        <rdfs:domain rdf:resource="http://semantic-web-kms.edu.et/wdo#DockerfileSpecification"/>
        <rdfs:range rdf:resource="http://semantic-web-kms.edu.et/wdo#ContainerImage"/>
        <rdfs:label xml:lang="en">is based on</rdfs:label>
        <skos:definition xml:lang="en">A relation from a Dockerfile specification to the base container image it extends.</skos:definition>
    </owl:ObjectProperty>
    


    <!-- http://semantic-web-kms.edu.et/wdo#isDependencyOf -->

    <owl:ObjectProperty rdf:about="http://semantic-web-kms.edu.et/wdo#isDependencyOf">
        <owl:inverseOf rdf:resource="http://semantic-web-kms.edu.et/wdo#specifiesDependency"/>
        <rdfs:domain rdf:resource="http://semantic-web-kms.edu.et/wdo#SoftwarePackage"/>
        <rdfs:range>
            <owl:Class>
                <owl:unionOf rdf:parseType="Collection">
                    <rdf:Description rdf:about="http://semantic-web-kms.edu.et/wdo#BuildScript"/>
                    <rdf:Description rdf:about="http://semantic-web-kms.edu.et/wdo#SoftwarePackage"/>
                </owl:unionOf>
            </owl:Class>
        </rdfs:range>
        <dc:identifier>WDO_OP:0000030</dc:identifier>
        <rdfs:label xml:lang="en">is dependency of</rdfs:label>
        <skos:definition xml:lang="en">A relation that is the inverse of &apos;specifiesDependency&apos;, indicating that a software package is a dependency of a build script or another package.</skos:definition>
    </owl:ObjectProperty>
    


    <!-- http://semantic-web-kms.edu.et/wdo#isDocumentedBy -->

    <owl:ObjectProperty rdf:about="http://semantic-web-kms.edu.et/wdo#isDocumentedBy">
        <rdfs:domain rdf:resource="http://purl.obolibrary.org/obo/BFO_0000001"/>
        <rdfs:range rdf:resource="http://semantic-web-kms.edu.et/wdo#Documentation"/>
        <rdfs:label xml:lang="en">is documented by</rdfs:label>
        <skos:definition xml:lang="en">Inverse of documentsEntity.</skos:definition>
    </owl:ObjectProperty>
    


    <!-- http://semantic-web-kms.edu.et/wdo#isElementOf -->

    <owl:ObjectProperty rdf:about="http://semantic-web-kms.edu.et/wdo#isElementOf">
        <rdfs:domain rdf:resource="http://semantic-web-kms.edu.et/wdo#InformationContentEntity"/>
        <rdfs:range rdf:resource="http://semantic-web-kms.edu.et/wdo#DigitalInformationCarrier"/>
        <dc:identifier>WDO_OP:0000036</dc:identifier>
        <rdfs:label xml:lang="en">is element of</rdfs:label>
        <skos:definition xml:lang="en">A relation indicating that an information content entity (e.g., a documentation segment or code construct) is part of a digital information carrier (file).</skos:definition>
    </owl:ObjectProperty>
    


    <!-- http://semantic-web-kms.edu.et/wdo#isImportedBy -->

    <owl:ObjectProperty rdf:about="http://semantic-web-kms.edu.et/wdo#isImportedBy">
        <rdfs:domain rdf:resource="http://semantic-web-kms.edu.et/wdo#Module"/>
        <rdfs:range rdf:resource="http://semantic-web-kms.edu.et/wdo#Module"/>
        <dc:identifier>WDO_OP:0000029</dc:identifier>
        <rdfs:label xml:lang="en">is imported by</rdfs:label>
        <skos:definition xml:lang="en">A relation that is the inverse of &apos;imports&apos;, indicating that a module&apos;s functionality is used by another module.</skos:definition>
    </owl:ObjectProperty>
    


    <!-- http://semantic-web-kms.edu.et/wdo#isMethodOf -->

    <owl:ObjectProperty rdf:about="http://semantic-web-kms.edu.et/wdo#isMethodOf">
        <rdfs:domain rdf:resource="http://semantic-web-kms.edu.et/wdo#FunctionDefinition"/>
        <rdfs:range rdf:resource="http://semantic-web-kms.edu.et/wdo#ComplexType"/>
        <rdfs:label xml:lang="en">is method of</rdfs:label>
        <skos:definition xml:lang="en">A relation that is the inverse of &apos;hasMethod&apos;, indicating that a function definition is a method of a specific class or interface.</skos:definition>
    </owl:ObjectProperty>
    


    <!-- http://semantic-web-kms.edu.et/wdo#isRelatedTo -->

    <owl:ObjectProperty rdf:about="http://semantic-web-kms.edu.et/wdo#isRelatedTo">
        <rdfs:domain rdf:resource="http://semantic-web-kms.edu.et/wdo#Issue"/>
        <rdfs:range rdf:resource="http://purl.obolibrary.org/obo/BFO_0000001"/>
        <rdfs:label xml:lang="en">is related to</rdfs:label>
        <skos:definition xml:lang="en">A general relation linking an issue to any relevant entity.</skos:definition>
    </owl:ObjectProperty>
    


    <!-- http://semantic-web-kms.edu.et/wdo#isTestedBy -->

    <owl:ObjectProperty rdf:about="http://semantic-web-kms.edu.et/wdo#isTestedBy">
        <owl:inverseOf rdf:resource="http://semantic-web-kms.edu.et/wdo#tests"/>
        <rdfs:domain rdf:resource="http://semantic-web-kms.edu.et/wdo#SoftwareCode"/>
        <rdfs:range rdf:resource="http://semantic-web-kms.edu.et/wdo#SoftwareCode"/>
        <dc:identifier>WDO_OP:0000032</dc:identifier>
        <rdfs:label xml:lang="en">is tested by</rdfs:label>
        <skos:definition xml:lang="en">A relation that is the inverse of &apos;tests&apos;, indicating that a piece of software code is verified by a set of test code.</skos:definition>
    </owl:ObjectProperty>
    


    <!-- http://semantic-web-kms.edu.et/wdo#justifies -->

    <owl:ObjectProperty rdf:about="http://semantic-web-kms.edu.et/wdo#justifies">
        <rdfs:domain rdf:resource="http://semantic-web-kms.edu.et/wdo#ArchitecturalDecisionRecord"/>
        <rdfs:range rdf:resource="http://purl.obolibrary.org/obo/BFO_0000001"/>
        <rdfs:label xml:lang="en">justifies</rdfs:label>
        <skos:definition xml:lang="en">Links an ADR to the architectural component or design choice it justifies.</skos:definition>
    </owl:ObjectProperty>
    


    <!-- http://semantic-web-kms.edu.et/wdo#manipulates -->

    <owl:ObjectProperty rdf:about="http://semantic-web-kms.edu.et/wdo#manipulates">
        <rdfs:domain rdf:resource="http://semantic-web-kms.edu.et/wdo#JavaScriptCode"/>
        <rdfs:range rdf:resource="http://semantic-web-kms.edu.et/wdo#HTMLCode"/>
        <dc:identifier>WDO_OP:0000019</dc:identifier>
        <rdfs:label xml:lang="en">manipulates</rdfs:label>
        <skos:definition xml:lang="en">A relation indicating that JavaScript code acts on or modifies HTML code, such as through the Document Object Model (DOM).</skos:definition>
    </owl:ObjectProperty>
    


    <!-- http://semantic-web-kms.edu.et/wdo#modifies -->

    <owl:ObjectProperty rdf:about="http://semantic-web-kms.edu.et/wdo#modifies">
        <rdfs:domain rdf:resource="http://semantic-web-kms.edu.et/wdo#Commit"/>
        <rdfs:range rdf:resource="http://semantic-web-kms.edu.et/wdo#DigitalInformationCarrier"/>
        <rdfs:label xml:lang="en">modifies</rdfs:label>
        <skos:definition xml:lang="en">A relation between a commit and the file(s) it changed.</skos:definition>
    </owl:ObjectProperty>
    


    <!-- http://semantic-web-kms.edu.et/wdo#packagesInto -->

    <owl:ObjectProperty rdf:about="http://semantic-web-kms.edu.et/wdo#packagesInto">
        <rdfs:domain rdf:resource="http://semantic-web-kms.edu.et/wdo#BuildScript"/>
        <rdfs:range rdf:resource="http://semantic-web-kms.edu.et/wdo#DigitalInformationCarrier"/>
        <rdfs:label xml:lang="en">packages into</rdfs:label>
        <skos:definition xml:lang="en">A relation from a build script to the final distributable artifact it creates (e.g., a JAR, a wheel).</skos:definition>
    </owl:ObjectProperty>
    


    <!-- http://semantic-web-kms.edu.et/wdo#queriesDatabase -->

    <owl:ObjectProperty rdf:about="http://semantic-web-kms.edu.et/wdo#queriesDatabase">
        <rdfs:domain rdf:resource="http://semantic-web-kms.edu.et/wdo#SQLCode"/>
        <rdfs:range rdf:resource="http://semantic-web-kms.edu.et/wdo#DatabaseSchema"/>
        <rdfs:label xml:lang="en">queries database</rdfs:label>
        <skos:definition xml:lang="en">A relation from an SQL query to the database schema it targets.</skos:definition>
    </owl:ObjectProperty>
    


    <!-- http://semantic-web-kms.edu.et/wdo#specifiesDependency -->

    <owl:ObjectProperty rdf:about="http://semantic-web-kms.edu.et/wdo#specifiesDependency">
        <rdfs:domain>
            <owl:Class>
                <owl:unionOf rdf:parseType="Collection">
                    <rdf:Description rdf:about="http://semantic-web-kms.edu.et/wdo#BuildScript"/>
                    <rdf:Description rdf:about="http://semantic-web-kms.edu.et/wdo#SoftwarePackage"/>
                </owl:unionOf>
            </owl:Class>
        </rdfs:domain>
        <rdfs:range rdf:resource="http://semantic-web-kms.edu.et/wdo#SoftwarePackage"/>
        <dc:identifier>WDO_OP:0000025</dc:identifier>
        <rdfs:label xml:lang="en">specifies dependency</rdfs:label>
        <skos:definition xml:lang="en">A relation indicating that a build script or software package specifies another package as a dependency.</skos:definition>
    </owl:ObjectProperty>
    


    <!-- http://semantic-web-kms.edu.et/wdo#styles -->

    <owl:ObjectProperty rdf:about="http://semantic-web-kms.edu.et/wdo#styles">
        <rdfs:domain rdf:resource="http://semantic-web-kms.edu.et/wdo#CSSCode"/>
        <rdfs:range rdf:resource="http://semantic-web-kms.edu.et/wdo#HTMLCode"/>
        <dc:identifier>WDO_OP:0000027</dc:identifier>
        <rdfs:label xml:lang="en">styles</rdfs:label>
        <skos:definition xml:lang="en">A relation indicating that a CSS entity provides presentation rules for an HTML entity.</skos:definition>
    </owl:ObjectProperty>
    


    <!-- http://semantic-web-kms.edu.et/wdo#tests -->

    <owl:ObjectProperty rdf:about="http://semantic-web-kms.edu.et/wdo#tests">
        <rdfs:domain rdf:resource="http://semantic-web-kms.edu.et/wdo#SoftwareCode"/>
        <rdfs:range rdf:resource="http://semantic-web-kms.edu.et/wdo#SoftwareCode"/>
        <dc:identifier>WDO_OP:0000031</dc:identifier>
        <rdfs:label xml:lang="en">tests</rdfs:label>
        <skos:definition xml:lang="en">A relation between code borne by a TestFile and the application code it is intended to verify.</skos:definition>
    </owl:ObjectProperty>
    


    <!-- http://semantic-web-kms.edu.et/wdo#usesFramework -->

    <owl:ObjectProperty rdf:about="http://semantic-web-kms.edu.et/wdo#usesFramework">
        <rdfs:domain rdf:resource="http://semantic-web-kms.edu.et/wdo#SoftwareCode"/>
        <rdfs:range rdf:resource="http://semantic-web-kms.edu.et/wdo#SoftwareFramework"/>
        <dc:identifier>WDO_OP:0000023</dc:identifier>
        <rdfs:label xml:lang="en">uses framework</rdfs:label>
        <skos:definition xml:lang="en">A relation indicating that a piece of software code is built upon or makes use of a software framework.</skos:definition>
    </owl:ObjectProperty>
    


    <!-- 
    ///////////////////////////////////////////////////////////////////////////////////////
    //
    // Data properties
    //
    ///////////////////////////////////////////////////////////////////////////////////////
     -->

    


    <!-- http://semantic-web-kms.edu.et/wdo#endsAtLine -->

    <owl:DatatypeProperty rdf:about="http://semantic-web-kms.edu.et/wdo#endsAtLine">
        <rdfs:domain rdf:resource="http://semantic-web-kms.edu.et/wdo#InformationContentEntity"/>
        <rdfs:range rdf:resource="http://www.w3.org/2001/XMLSchema#nonNegativeInteger"/>
        <dc:identifier>WDO_DP:0000003</dc:identifier>
        <rdfs:label xml:lang="en">ends at line</rdfs:label>
        <skos:definition xml:lang="en">A data property that specifies the ending line number of a code or document element within its source file.</skos:definition>
    </owl:DatatypeProperty>
    


    <!-- http://semantic-web-kms.edu.et/wdo#hasAccessModifier -->

    <owl:DatatypeProperty rdf:about="http://semantic-web-kms.edu.et/wdo#hasAccessModifier">
        <rdfs:domain rdf:resource="http://semantic-web-kms.edu.et/wdo#AttributeDeclaration"/>
        <rdfs:range rdf:resource="http://www.w3.org/2001/XMLSchema#string"/>
        <rdfs:label xml:lang="en">has access modifier</rdfs:label>
        <skos:definition xml:lang="en">The visibility of a field or method (e.g., &quot;public&quot;, &quot;private&quot;).</skos:definition>
    </owl:DatatypeProperty>
    


    <!-- http://semantic-web-kms.edu.et/wdo#hasCanonicalName -->

    <owl:DatatypeProperty rdf:about="http://semantic-web-kms.edu.et/wdo#hasCanonicalName">
        <rdfs:domain rdf:resource="http://semantic-web-kms.edu.et/wdo#SoftwareCode"/>
        <rdfs:range rdf:resource="http://www.w3.org/2001/XMLSchema#string"/>
        <dc:identifier>WDO_DP:0000004</dc:identifier>
        <rdfs:label xml:lang="en">has canonical name</rdfs:label>
        <skos:definition xml:lang="en">A data property that specifies the fully qualified or canonical name of a code element (e.g., package.class.method).</skos:definition>
    </owl:DatatypeProperty>
    


    <!-- http://semantic-web-kms.edu.et/wdo#hasCategory -->

    <owl:DatatypeProperty rdf:about="http://semantic-web-kms.edu.et/wdo#hasCategory">
        <rdfs:domain rdf:resource="http://semantic-web-kms.edu.et/wdo#DigitalInformationCarrier"/>
        <rdfs:range rdf:resource="http://www.w3.org/2001/XMLSchema#string"/>
        <dc:identifier>WDO_DP:0000021</dc:identifier>
        <rdfs:label xml:lang="en">has category</rdfs:label>
        <skos:definition xml:lang="en">A data property that specifies the category or type of a digital information carrier (e.g., code, asset, configuration).</skos:definition>
    </owl:DatatypeProperty>
    


    <!-- http://semantic-web-kms.edu.et/wdo#hasCommitHash -->

    <owl:DatatypeProperty rdf:about="http://semantic-web-kms.edu.et/wdo#hasCommitHash">
        <rdfs:domain rdf:resource="http://semantic-web-kms.edu.et/wdo#Commit"/>
        <rdfs:range rdf:resource="http://www.w3.org/2001/XMLSchema#string"/>
        <rdfs:label xml:lang="en">has commit hash</rdfs:label>
        <skos:definition xml:lang="en">The unique SHA hash identifying a commit.</skos:definition>
    </owl:DatatypeProperty>
    


    <!-- http://semantic-web-kms.edu.et/wdo#hasContent -->

    <owl:DatatypeProperty rdf:about="http://semantic-web-kms.edu.et/wdo#hasContent">
        <rdfs:domain rdf:resource="http://semantic-web-kms.edu.et/wdo#InformationContentEntity"/>
        <rdfs:range rdf:resource="http://www.w3.org/2001/XMLSchema#string"/>
        <dc:identifier>WDO_DP:0000020</dc:identifier>
        <rdfs:label xml:lang="en">has content</rdfs:label>
        <skos:definition xml:lang="en">A data property that holds the literal content or value of an information entity, such as a configuration setting or documentation segment.</skos:definition>
    </owl:DatatypeProperty>
    


    <!-- http://semantic-web-kms.edu.et/wdo#hasCreationTimestamp -->

    <owl:DatatypeProperty rdf:about="http://semantic-web-kms.edu.et/wdo#hasCreationTimestamp">
        <rdfs:domain rdf:resource="http://semantic-web-kms.edu.et/wdo#DigitalInformationCarrier"/>
        <rdfs:range rdf:resource="http://www.w3.org/2001/XMLSchema#dateTime"/>
        <rdfs:label xml:lang="en">has creation timestamp</rdfs:label>
        <skos:definition xml:lang="en">The timestamp when a file was first created.</skos:definition>
    </owl:DatatypeProperty>
    


    <!-- http://semantic-web-kms.edu.et/wdo#hasCyclomaticComplexity -->

    <owl:DatatypeProperty rdf:about="http://semantic-web-kms.edu.et/wdo#hasCyclomaticComplexity">
        <rdfs:domain rdf:resource="http://semantic-web-kms.edu.et/wdo#FunctionDefinition"/>
        <rdfs:range rdf:resource="http://www.w3.org/2001/XMLSchema#positiveInteger"/>
        <rdfs:label xml:lang="en">has cyclomatic complexity</rdfs:label>
        <skos:definition xml:lang="en">A standard measure of code complexity.</skos:definition>
    </owl:DatatypeProperty>
    


    <!-- http://semantic-web-kms.edu.et/wdo#hasEndpointPath -->

    <owl:DatatypeProperty rdf:about="http://semantic-web-kms.edu.et/wdo#hasEndpointPath">
        <rdfs:domain rdf:resource="http://semantic-web-kms.edu.et/wdo#APIDocumentation"/>
        <rdfs:range rdf:resource="http://www.w3.org/2001/XMLSchema#string"/>
        <rdfs:label xml:lang="en">has endpoint path</rdfs:label>
        <skos:definition xml:lang="en">The URL path for an API endpoint.</skos:definition>
    </owl:DatatypeProperty>
    


    <!-- http://semantic-web-kms.edu.et/wdo#hasExtension -->

    <owl:DatatypeProperty rdf:about="http://semantic-web-kms.edu.et/wdo#hasExtension">
        <rdfs:domain rdf:resource="http://semantic-web-kms.edu.et/wdo#DigitalInformationCarrier"/>
        <rdfs:range rdf:resource="http://www.w3.org/2001/XMLSchema#string"/>
        <dc:identifier>WDO_DP:0000022</dc:identifier>
        <rdfs:label xml:lang="en">has extension</rdfs:label>
        <skos:definition xml:lang="en">A data property that specifies the file extension of a digital information carrier (e.g., &apos;py&apos;, &apos;md&apos;, &apos;png&apos;).</skos:definition>
    </owl:DatatypeProperty>
    


    <!-- http://semantic-web-kms.edu.et/wdo#hasFontFamilyName -->

    <owl:DatatypeProperty rdf:about="http://semantic-web-kms.edu.et/wdo#hasFontFamilyName">
        <rdfs:domain rdf:resource="http://semantic-web-kms.edu.et/wdo#FontDescription"/>
        <rdfs:range rdf:resource="http://www.w3.org/2001/XMLSchema#string"/>
        <dc:identifier>WDO_DP:0000014</dc:identifier>
        <rdfs:label xml:lang="en">has font family name</rdfs:label>
        <skos:definition xml:lang="en">The family name of a font (e.g., Arial, Times New Roman).</skos:definition>
    </owl:DatatypeProperty>
    


    <!-- http://semantic-web-kms.edu.et/wdo#hasFontStyle -->

    <owl:DatatypeProperty rdf:about="http://semantic-web-kms.edu.et/wdo#hasFontStyle">
        <rdfs:domain rdf:resource="http://semantic-web-kms.edu.et/wdo#FontDescription"/>
        <rdfs:range rdf:resource="http://www.w3.org/2001/XMLSchema#string"/>
        <dc:identifier>WDO_DP:0000015</dc:identifier>
        <rdfs:label xml:lang="en">has font style</rdfs:label>
        <skos:definition xml:lang="en">The style of a font (e.g., Regular, Italic, Bold).</skos:definition>
    </owl:DatatypeProperty>
    


    <!-- http://semantic-web-kms.edu.et/wdo#hasFrameRate -->

    <owl:DatatypeProperty rdf:about="http://semantic-web-kms.edu.et/wdo#hasFrameRate">
        <rdfs:domain rdf:resource="http://semantic-web-kms.edu.et/wdo#VideoDescription"/>
        <rdfs:range rdf:resource="http://www.w3.org/2001/XMLSchema#decimal"/>
        <dc:identifier>WDO_DP:0000011</dc:identifier>
        <rdfs:label xml:lang="en">has frame rate</rdfs:label>
        <skos:definition xml:lang="en">The frame rate of a video asset in frames per second.</skos:definition>
    </owl:DatatypeProperty>
    


    <!-- http://semantic-web-kms.edu.et/wdo#hasHeadingLevel -->

    <owl:DatatypeProperty rdf:about="http://semantic-web-kms.edu.et/wdo#hasHeadingLevel">
        <rdfs:domain rdf:resource="http://semantic-web-kms.edu.et/wdo#Heading"/>
        <rdfs:range rdf:resource="http://www.w3.org/2001/XMLSchema#positiveInteger"/>
        <dc:identifier>WDO_DP:0000016</dc:identifier>
        <rdfs:label xml:lang="en">has heading level</rdfs:label>
        <skos:definition xml:lang="en">A data property that specifies the hierarchical level of a heading in a document (e.g., 1 for &lt;h1&gt;, 2 for &lt;h2&gt;).</skos:definition>
    </owl:DatatypeProperty>
    


    <!-- http://semantic-web-kms.edu.et/wdo#hasHttpMethod -->

    <owl:DatatypeProperty rdf:about="http://semantic-web-kms.edu.et/wdo#hasHttpMethod">
        <rdfs:domain rdf:resource="http://semantic-web-kms.edu.et/wdo#APIDocumentation"/>
        <rdfs:range rdf:resource="http://www.w3.org/2001/XMLSchema#string"/>
        <rdfs:label xml:lang="en">has http method</rdfs:label>
        <skos:definition xml:lang="en">The allowed HTTP method for an API endpoint (e.g., &quot;GET&quot;, &quot;POST&quot;).</skos:definition>
    </owl:DatatypeProperty>
    


    <!-- http://semantic-web-kms.edu.et/wdo#hasImageFormatName -->

    <owl:DatatypeProperty rdf:about="http://semantic-web-kms.edu.et/wdo#hasImageFormatName">
        <rdfs:domain rdf:resource="http://semantic-web-kms.edu.et/wdo#ImageDescription"/>
        <rdfs:range rdf:resource="http://www.w3.org/2001/XMLSchema#string"/>
        <dc:identifier>WDO_DP:0000009</dc:identifier>
        <rdfs:label xml:lang="en">has image format name</rdfs:label>
        <skos:definition xml:lang="en">The common name of the image format (e.g., JPEG, PNG, SVG).</skos:definition>
    </owl:DatatypeProperty>
    


    <!-- http://semantic-web-kms.edu.et/wdo#hasImageHeight -->

    <owl:DatatypeProperty rdf:about="http://semantic-web-kms.edu.et/wdo#hasImageHeight">
        <rdfs:domain rdf:resource="http://semantic-web-kms.edu.et/wdo#ImageDescription"/>
        <rdfs:range rdf:resource="http://www.w3.org/2001/XMLSchema#nonNegativeInteger"/>
        <dc:identifier>WDO_DP:0000008</dc:identifier>
        <rdfs:label xml:lang="en">has image height</rdfs:label>
        <skos:definition xml:lang="en">The height of the image in pixels.</skos:definition>
    </owl:DatatypeProperty>
    


    <!-- http://semantic-web-kms.edu.et/wdo#hasImageWidth -->

    <owl:DatatypeProperty rdf:about="http://semantic-web-kms.edu.et/wdo#hasImageWidth">
        <rdfs:domain rdf:resource="http://semantic-web-kms.edu.et/wdo#ImageDescription"/>
        <rdfs:range rdf:resource="http://www.w3.org/2001/XMLSchema#nonNegativeInteger"/>
        <dc:identifier>WDO_DP:0000007</dc:identifier>
        <rdfs:label xml:lang="en">has image width</rdfs:label>
        <skos:definition xml:lang="en">The width of the image in pixels.</skos:definition>
    </owl:DatatypeProperty>
    


    <!-- http://semantic-web-kms.edu.et/wdo#hasIssueIdentifier -->

    <owl:DatatypeProperty rdf:about="http://semantic-web-kms.edu.et/wdo#hasIssueIdentifier">
        <rdfs:domain rdf:resource="http://semantic-web-kms.edu.et/wdo#Issue"/>
        <rdfs:range rdf:resource="http://www.w3.org/2001/XMLSchema#string"/>
        <rdfs:label xml:lang="en">has issue identifier</rdfs:label>
        <skos:definition xml:lang="en">The ID from the issue tracking system.</skos:definition>
    </owl:DatatypeProperty>
    


    <!-- http://semantic-web-kms.edu.et/wdo#hasLicenseIdentifier -->

    <owl:DatatypeProperty rdf:about="http://semantic-web-kms.edu.et/wdo#hasLicenseIdentifier">
        <rdfs:domain rdf:resource="http://semantic-web-kms.edu.et/wdo#License"/>
        <rdfs:range rdf:resource="http://www.w3.org/2001/XMLSchema#string"/>
        <dc:identifier>WDO_DP:0000018</dc:identifier>
        <rdfs:label xml:lang="en">has license identifier</rdfs:label>
        <skos:definition xml:lang="en">A data property that specifies the standard identifier for a license, preferably its SPDX ID (e.g., &quot;MIT&quot;, &quot;Apache-2.0&quot;).</skos:definition>
    </owl:DatatypeProperty>
    


    <!-- http://semantic-web-kms.edu.et/wdo#hasLineCount -->

    <owl:DatatypeProperty rdf:about="http://semantic-web-kms.edu.et/wdo#hasLineCount">
        <rdfs:domain rdf:resource="http://semantic-web-kms.edu.et/wdo#SoftwareCode"/>
        <rdfs:range rdf:resource="http://www.w3.org/2001/XMLSchema#nonNegativeInteger"/>
        <rdfs:label xml:lang="en">has line count</rdfs:label>
        <skos:definition xml:lang="en">The number of lines in a piece of code.</skos:definition>
    </owl:DatatypeProperty>
    


    <!-- http://semantic-web-kms.edu.et/wdo#hasMediaDuration -->

    <owl:DatatypeProperty rdf:about="http://semantic-web-kms.edu.et/wdo#hasMediaDuration">
        <rdfs:domain>
            <owl:Class>
                <owl:unionOf rdf:parseType="Collection">
                    <rdf:Description rdf:about="http://semantic-web-kms.edu.et/wdo#AudioDescription"/>
                    <rdf:Description rdf:about="http://semantic-web-kms.edu.et/wdo#VideoDescription"/>
                </owl:unionOf>
            </owl:Class>
        </rdfs:domain>
        <rdfs:range rdf:resource="http://www.w3.org/2001/XMLSchema#duration"/>
        <dc:identifier>WDO_DP:0000010</dc:identifier>
        <rdfs:label xml:lang="en">has media duration</rdfs:label>
        <skos:definition xml:lang="en">The duration of a time-based media asset, such as video or audio.</skos:definition>
    </owl:DatatypeProperty>
    


    <!-- http://semantic-web-kms.edu.et/wdo#hasMediaEncodingFormat -->

    <owl:DatatypeProperty rdf:about="http://semantic-web-kms.edu.et/wdo#hasMediaEncodingFormat">
        <rdfs:domain>
            <owl:Class>
                <owl:unionOf rdf:parseType="Collection">
                    <rdf:Description rdf:about="http://semantic-web-kms.edu.et/wdo#AudioDescription"/>
                    <rdf:Description rdf:about="http://semantic-web-kms.edu.et/wdo#VideoDescription"/>
                </owl:unionOf>
            </owl:Class>
        </rdfs:domain>
        <rdfs:range rdf:resource="http://www.w3.org/2001/XMLSchema#string"/>
        <dc:identifier>WDO_DP:0000012</dc:identifier>
        <rdfs:label xml:lang="en">has media encoding format</rdfs:label>
        <skos:definition xml:lang="en">The encoding format of a media asset (e.g., H.264 for video, AAC for audio).</skos:definition>
    </owl:DatatypeProperty>
    


    <!-- http://semantic-web-kms.edu.et/wdo#hasModificationTimestamp -->

    <owl:DatatypeProperty rdf:about="http://semantic-web-kms.edu.et/wdo#hasModificationTimestamp">
        <rdfs:domain rdf:resource="http://semantic-web-kms.edu.et/wdo#DigitalInformationCarrier"/>
        <rdfs:range rdf:resource="http://www.w3.org/2001/XMLSchema#dateTime"/>
        <rdfs:label xml:lang="en">has modification timestamp</rdfs:label>
        <skos:definition xml:lang="en">The timestamp when a file was last modified.</skos:definition>
    </owl:DatatypeProperty>
    


    <!-- http://semantic-web-kms.edu.et/wdo#hasRelativePath -->

    <owl:DatatypeProperty rdf:about="http://semantic-web-kms.edu.et/wdo#hasRelativePath">
        <rdfs:domain rdf:resource="http://semantic-web-kms.edu.et/wdo#DigitalInformationCarrier"/>
        <rdfs:range rdf:resource="http://www.w3.org/2001/XMLSchema#string"/>
        <dc:identifier>WDO_DP:0000017</dc:identifier>
        <rdfs:label xml:lang="en">has relative path</rdfs:label>
        <skos:definition xml:lang="en">A data property that specifies the path of a file relative to the root of its source repository.</skos:definition>
    </owl:DatatypeProperty>
    


    <!-- http://semantic-web-kms.edu.et/wdo#hasSampleRate -->

    <owl:DatatypeProperty rdf:about="http://semantic-web-kms.edu.et/wdo#hasSampleRate">
        <rdfs:domain rdf:resource="http://semantic-web-kms.edu.et/wdo#AudioDescription"/>
        <rdfs:range rdf:resource="http://www.w3.org/2001/XMLSchema#decimal"/>
        <dc:identifier>WDO_DP:0000013</dc:identifier>
        <rdfs:label xml:lang="en">has sample rate</rdfs:label>
        <skos:definition xml:lang="en">The sample rate of an audio asset in Hertz (Hz).</skos:definition>
    </owl:DatatypeProperty>
    


    <!-- http://semantic-web-kms.edu.et/wdo#hasSimpleName -->

    <owl:DatatypeProperty rdf:about="http://semantic-web-kms.edu.et/wdo#hasSimpleName">
        <rdfs:domain rdf:resource="http://semantic-web-kms.edu.et/wdo#InformationContentEntity"/>
        <rdfs:range rdf:resource="http://www.w3.org/2001/XMLSchema#string"/>
        <dc:identifier>WDO_DP:0000005</dc:identifier>
        <rdfs:label xml:lang="en">has simple name</rdfs:label>
        <skos:definition xml:lang="en">A data property that specifies the simple, unqualified name of a code or document element.</skos:definition>
    </owl:DatatypeProperty>
    


    <!-- http://semantic-web-kms.edu.et/wdo#hasSizeInBytes -->

    <owl:DatatypeProperty rdf:about="http://semantic-web-kms.edu.et/wdo#hasSizeInBytes">
        <rdfs:domain rdf:resource="http://semantic-web-kms.edu.et/wdo#DigitalInformationCarrier"/>
        <rdfs:range rdf:resource="http://www.w3.org/2001/XMLSchema#nonNegativeInteger"/>
        <dc:identifier>WDO_DP:0000019</dc:identifier>
        <rdfs:label xml:lang="en">has size in bytes</rdfs:label>
        <skos:definition xml:lang="en">A data property that specifies the size of a file in bytes.</skos:definition>
    </owl:DatatypeProperty>
    


    <!-- http://semantic-web-kms.edu.et/wdo#hasSourceCodeSnippet -->

    <owl:DatatypeProperty rdf:about="http://semantic-web-kms.edu.et/wdo#hasSourceCodeSnippet">
        <rdfs:domain rdf:resource="http://semantic-web-kms.edu.et/wdo#SoftwareCode"/>
        <rdfs:range rdf:resource="http://www.w3.org/2001/XMLSchema#string"/>
        <dc:identifier>WDO_DP:0000001</dc:identifier>
        <rdfs:label xml:lang="en">has source code snippet</rdfs:label>
        <skos:definition xml:lang="en">A data property that holds the literal source code string of a SoftwareCode element.</skos:definition>
    </owl:DatatypeProperty>
    


    <!-- http://semantic-web-kms.edu.et/wdo#hasStatus -->

    <owl:DatatypeProperty rdf:about="http://semantic-web-kms.edu.et/wdo#hasStatus">
        <rdfs:domain rdf:resource="http://semantic-web-kms.edu.et/wdo#Issue"/>
        <rdfs:range rdf:resource="http://www.w3.org/2001/XMLSchema#string"/>
        <rdfs:label xml:lang="en">has status</rdfs:label>
        <skos:definition xml:lang="en">The current state of an issue (e.g., &quot;Open&quot;, &quot;Resolved&quot;).</skos:definition>
    </owl:DatatypeProperty>
    


    <!-- http://semantic-web-kms.edu.et/wdo#hasTextValue -->

    <owl:DatatypeProperty rdf:about="http://semantic-web-kms.edu.et/wdo#hasTextValue">
        <rdfs:domain rdf:resource="http://semantic-web-kms.edu.et/wdo#TextualElement"/>
        <rdfs:range rdf:resource="http://www.w3.org/2001/XMLSchema#string"/>
        <dc:identifier>WDO_DP:0000006</dc:identifier>
        <rdfs:label xml:lang="en">has text value</rdfs:label>
        <skos:definition xml:lang="en">A data property that holds the literal text value of a textual document component.</skos:definition>
    </owl:DatatypeProperty>
    


    <!-- http://semantic-web-kms.edu.et/wdo#hasVersion -->

    <owl:DatatypeProperty rdf:about="http://semantic-web-kms.edu.et/wdo#hasVersion">
        <rdfs:domain>
            <owl:Class>
                <owl:unionOf rdf:parseType="Collection">
                    <rdf:Description rdf:about="http://semantic-web-kms.edu.et/wdo#SoftwareFramework"/>
                    <rdf:Description rdf:about="http://semantic-web-kms.edu.et/wdo#SoftwarePackage"/>
                </owl:unionOf>
            </owl:Class>
        </rdfs:domain>
        <rdfs:range rdf:resource="http://www.w3.org/2001/XMLSchema#string"/>
        <dc:identifier>WDO_DP:0000020</dc:identifier>
        <rdfs:label xml:lang="en">has version</rdfs:label>
        <skos:definition xml:lang="en">A data property that specifies the version string of a software package or framework (e.g., &quot;16.8.0&quot;, &quot;5.2.3&quot;).</skos:definition>
    </owl:DatatypeProperty>
    


    <!-- http://semantic-web-kms.edu.et/wdo#isAsynchronous -->

    <owl:DatatypeProperty rdf:about="http://semantic-web-kms.edu.et/wdo#isAsynchronous">
        <rdfs:domain rdf:resource="http://semantic-web-kms.edu.et/wdo#FunctionDefinition"/>
        <rdfs:range rdf:resource="http://www.w3.org/2001/XMLSchema#boolean"/>
        <rdfs:label xml:lang="en">is asynchronous</rdfs:label>
        <skos:definition xml:lang="en">A flag indicating if a function is asynchronous.</skos:definition>
    </owl:DatatypeProperty>
    


    <!-- http://semantic-web-kms.edu.et/wdo#startsAtLine -->

    <owl:DatatypeProperty rdf:about="http://semantic-web-kms.edu.et/wdo#startsAtLine">
        <rdfs:domain rdf:resource="http://semantic-web-kms.edu.et/wdo#InformationContentEntity"/>
        <rdfs:range rdf:resource="http://www.w3.org/2001/XMLSchema#nonNegativeInteger"/>
        <dc:identifier>WDO_DP:0000002</dc:identifier>
        <rdfs:label xml:lang="en">starts at line</rdfs:label>
        <skos:definition xml:lang="en">A data property that specifies the starting line number of a code or document element within its source file.</skos:definition>
    </owl:DatatypeProperty>
    


    <!-- 
    ///////////////////////////////////////////////////////////////////////////////////////
    //
    // Classes
    //
    ///////////////////////////////////////////////////////////////////////////////////////
     -->

    


    <!-- http://purl.obolibrary.org/obo/BFO_0000001 -->

    <owl:Class rdf:about="http://purl.obolibrary.org/obo/BFO_0000001"/>
    


    <!-- http://purl.obolibrary.org/obo/BFO_0000015 -->

    <owl:Class rdf:about="http://purl.obolibrary.org/obo/BFO_0000015"/>
    


    <!-- http://purl.obolibrary.org/obo/BFO_0000031 -->

    <owl:Class rdf:about="http://purl.obolibrary.org/obo/BFO_0000031"/>
    


    <!-- http://purl.obolibrary.org/obo/BFO_0000040 -->

    <owl:Class rdf:about="http://purl.obolibrary.org/obo/BFO_0000040"/>
    


    <!-- http://semantic-web-kms.edu.et/wdo#APIDocumentation -->

    <owl:Class rdf:about="http://semantic-web-kms.edu.et/wdo#APIDocumentation">
        <rdfs:subClassOf rdf:resource="http://semantic-web-kms.edu.et/wdo#Documentation"/>
        <dc:identifier>WDO:0000081</dc:identifier>
        <rdfs:label xml:lang="en">API Documentation</rdfs:label>
        <skos:definition xml:lang="en">A type of Documentation that describes an Application Programming Interface (API), including its endpoints, methods, parameters, and return values.</skos:definition>
        <skos:example xml:lang="en">A specification generated by Swagger/OpenAPI; documentation for a REST or GraphQL API.</skos:example>
    </owl:Class>
    


    <!-- http://semantic-web-kms.edu.et/wdo#ArchitecturalDecisionRecord -->

    <owl:Class rdf:about="http://semantic-web-kms.edu.et/wdo#ArchitecturalDecisionRecord">
        <rdfs:subClassOf rdf:resource="http://semantic-web-kms.edu.et/wdo#Documentation"/>
        <dc:identifier>WDO:0000082</dc:identifier>
        <rdfs:label xml:lang="en">Architectural Decision Record</rdfs:label>
        <skos:definition xml:lang="en">A type of Documentation that captures an important architectural decision made along with its context and consequences.</skos:definition>
    </owl:Class>
    


    <!-- http://semantic-web-kms.edu.et/wdo#ArchiveFile -->

    <owl:Class rdf:about="http://semantic-web-kms.edu.et/wdo#ArchiveFile">
        <rdfs:subClassOf rdf:resource="http://semantic-web-kms.edu.et/wdo#DigitalInformationCarrier"/>
        <dc:identifier>WDO:0000111</dc:identifier>
        <rdfs:label xml:lang="en">Archive File</rdfs:label>
        <skos:definition xml:lang="en">An ArchiveFile is a DigitalInformationCarrier that contains one or more files and is used for packaging, compression, or backup purposes.</skos:definition>
        <skos:example xml:lang="en">A file named &apos;project.zip&apos;, &apos;backup.tar.gz&apos;, or &apos;archive.7z&apos;.</skos:example>
    </owl:Class>
    


    <!-- http://semantic-web-kms.edu.et/wdo#AssetFile -->

    <owl:Class rdf:about="http://semantic-web-kms.edu.et/wdo#AssetFile">
        <rdfs:subClassOf rdf:resource="http://semantic-web-kms.edu.et/wdo#DigitalInformationCarrier"/>
        <owl:disjointWith rdf:resource="http://semantic-web-kms.edu.et/wdo#SourceCodeFile"/>
        <dc:identifier>WDO:0000036</dc:identifier>
        <rdfs:label xml:lang="en">Asset File</rdfs:label>
        <skos:definition xml:lang="en">An Asset File is a DigitalInformationCarrier that bears the description or content of a non-code, non-documentation digital resource used within a web development project, such as images, videos, audio files, or fonts. This is an abstract class for specific asset file types.</skos:definition>
        <skos:example xml:lang="en">An image file &apos;hero-banner.jpg&apos;; an audio file &apos;notification.mp3&apos;; a font file &apos;Roboto-Regular.ttf&apos;.</skos:example>
    </owl:Class>
    


    <!-- http://semantic-web-kms.edu.et/wdo#AttributeDeclaration -->

    <owl:Class rdf:about="http://semantic-web-kms.edu.et/wdo#AttributeDeclaration">
        <rdfs:subClassOf rdf:resource="http://semantic-web-kms.edu.et/wdo#SoftwareCode"/>
        <dc:identifier>WDO:0000010</dc:identifier>
        <rdfs:label xml:lang="en">Attribute Declaration</rdfs:label>
        <skos:definition xml:lang="en">An AttributeDeclaration is a SoftwareCode entity which is the declaration of an attribute, field, or property within a class or interface.</skos:definition>
        <skos:example xml:lang="en">The declaration &apos;private String username;&apos; within a class definition; &apos;const API_KEY = &quot;...&quot;&apos; in a JavaScript module.</skos:example>
    </owl:Class>
    


    <!-- http://semantic-web-kms.edu.et/wdo#AudioDescription -->

    <owl:Class rdf:about="http://semantic-web-kms.edu.et/wdo#AudioDescription">
        <rdfs:subClassOf rdf:resource="http://semantic-web-kms.edu.et/wdo#DigitalAssetDescription"/>
        <dc:identifier>WDO:0000026</dc:identifier>
        <rdfs:label xml:lang="en">Audio Description</rdfs:label>
        <skos:definition xml:lang="en">An AudioDescription is a DigitalAssetDescription which represents the informational nature of an audio recording, such as its duration, sample rate, and encoding.</skos:definition>
        <skos:example xml:lang="en">The informational content of a background music track, including its mood, tempo, and licensing terms; the description for a button click sound effect in MP3 format.</skos:example>
    </owl:Class>
    


    <!-- http://semantic-web-kms.edu.et/wdo#AudioFile -->

    <owl:Class rdf:about="http://semantic-web-kms.edu.et/wdo#AudioFile">
        <rdfs:subClassOf rdf:resource="http://semantic-web-kms.edu.et/wdo#AssetFile"/>
        <dc:identifier>WDO:0000039</dc:identifier>
        <rdfs:label xml:lang="en">Audio File</rdfs:label>
        <skos:definition xml:lang="en">An AudioFile is an AssetFile that bears an AudioDescription.</skos:definition>
        <skos:example xml:lang="en">A file named &apos;ui_click.wav&apos; or &apos;theme_song.ogg&apos;.</skos:example>
    </owl:Class>
    


    <!-- http://semantic-web-kms.edu.et/wdo#BestPracticeGuideline -->

    <owl:Class rdf:about="http://semantic-web-kms.edu.et/wdo#BestPracticeGuideline">
        <rdfs:subClassOf rdf:resource="http://semantic-web-kms.edu.et/wdo#Documentation"/>
        <dc:identifier>WDO:0000021</dc:identifier>
        <rdfs:label xml:lang="en">Best Practice Guideline</rdfs:label>
        <skos:definition xml:lang="en">A BestPracticeGuideline is a type of Documentation that describes recommended methods or techniques for web development.</skos:definition>
        <skos:example xml:lang="en">A document outlining &apos;Secure Coding Practices for Web Applications&apos;; a style guide for writing maintainable CSS; guidelines for REST API design.</skos:example>
    </owl:Class>
    


    <!-- http://semantic-web-kms.edu.et/wdo#Blockquote -->

    <owl:Class rdf:about="http://semantic-web-kms.edu.et/wdo#Blockquote">
        <rdfs:subClassOf rdf:resource="http://semantic-web-kms.edu.et/wdo#TextualElement"/>
        <dc:identifier>WDO:0000057</dc:identifier>
        <rdfs:label xml:lang="en">Blockquote</rdfs:label>
        <skos:definition xml:lang="en">A Blockquote is a TextualElement which consists of a block of quoted text, typically indented from the main text.</skos:definition>
        <skos:example xml:lang="en">A customer testimonial quoted in a README file, often prefixed with &apos;&gt;&apos; in Markdown.</skos:example>
    </owl:Class>
    


    <!-- http://semantic-web-kms.edu.et/wdo#BuildFile -->

    <owl:Class rdf:about="http://semantic-web-kms.edu.et/wdo#BuildFile">
        <rdfs:subClassOf rdf:resource="http://semantic-web-kms.edu.et/wdo#DigitalInformationCarrier"/>
        <dc:identifier>WDO:0000049</dc:identifier>
        <rdfs:label xml:lang="en">Build File</rdfs:label>
        <skos:definition xml:lang="en">A BuildFile is a DigitalInformationCarrier that bears a BuildScript, defining tasks for compiling, packaging, and deploying a software project.</skos:definition>
        <skos:example xml:lang="en">A file named &apos;pom.xml&apos; (Maven), &apos;build.gradle&apos; (Gradle), or &apos;Makefile&apos;.</skos:example>
    </owl:Class>
    


    <!-- http://semantic-web-kms.edu.et/wdo#BuildScript -->

    <owl:Class rdf:about="http://semantic-web-kms.edu.et/wdo#BuildScript">
        <rdfs:subClassOf rdf:resource="http://semantic-web-kms.edu.et/wdo#InformationContentEntity"/>
        <dc:identifier>WDO:0000070</dc:identifier>
        <rdfs:label xml:lang="en">Build Script</rdfs:label>
        <skos:definition xml:lang="en">A BuildScript is an InformationContentEntity which specifies the instructions and dependencies for a build system.</skos:definition>
        <skos:example xml:lang="en">The XML content of a pom.xml file defining project dependencies; the Groovy script within a build.gradle file.</skos:example>
    </owl:Class>
    


    <!-- http://semantic-web-kms.edu.et/wdo#CSSCode -->

    <owl:Class rdf:about="http://semantic-web-kms.edu.et/wdo#CSSCode">
        <rdfs:subClassOf rdf:resource="http://semantic-web-kms.edu.et/wdo#Stylesheet"/>
        <dc:identifier>WDO:0000076</dc:identifier>
        <rdfs:label xml:lang="en">CSS Code</rdfs:label>
        <skos:definition xml:lang="en">Software code written in the Cascading Style Sheets (CSS) language.</skos:definition>
    </owl:Class>
    


    <!-- http://semantic-web-kms.edu.et/wdo#CSSFramework -->

    <owl:Class rdf:about="http://semantic-web-kms.edu.et/wdo#CSSFramework">
        <rdfs:subClassOf rdf:resource="http://semantic-web-kms.edu.et/wdo#SoftwareFramework"/>
        <dc:identifier>WDO:0000093</dc:identifier>
        <rdfs:label xml:lang="en">CSS Framework</rdfs:label>
        <skos:definition xml:lang="en">A software framework that provides a collection of pre-written CSS files and other assets to facilitate easier, more standards-compliant web design.</skos:definition>
        <skos:example xml:lang="en">Bootstrap, Foundation, Tailwind CSS.</skos:example>
    </owl:Class>
    


    <!-- http://semantic-web-kms.edu.et/wdo#CSharpCode -->

    <owl:Class rdf:about="http://semantic-web-kms.edu.et/wdo#CSharpCode">
        <rdfs:subClassOf rdf:resource="http://semantic-web-kms.edu.et/wdo#StaticallyTypedLanguageCode"/>
        <dc:identifier>WDO:0000101</dc:identifier>
        <rdfs:label xml:lang="en">C# Code</rdfs:label>
        <skos:definition xml:lang="en">Software code written in the C# programming language, commonly used in enterprise web applications with the .NET framework.</skos:definition>
    </owl:Class>
    


    <!-- http://semantic-web-kms.edu.et/wdo#Changelog -->

    <owl:Class rdf:about="http://semantic-web-kms.edu.et/wdo#Changelog">
        <rdfs:subClassOf rdf:resource="http://semantic-web-kms.edu.et/wdo#Documentation"/>
        <dc:identifier>WDO:0000083</dc:identifier>
        <rdfs:label xml:lang="en">Changelog</rdfs:label>
        <skos:definition xml:lang="en">A type of Documentation that consists of a chronologically ordered list of notable changes made to a project.</skos:definition>
    </owl:Class>
    


    <!-- http://semantic-web-kms.edu.et/wdo#ClassDefinition -->

    <owl:Class rdf:about="http://semantic-web-kms.edu.et/wdo#ClassDefinition">
        <rdfs:subClassOf rdf:resource="http://semantic-web-kms.edu.et/wdo#ComplexType"/>
        <dc:identifier>WDO:0000007</dc:identifier>
        <rdfs:label xml:lang="en">Class Definition</rdfs:label>
        <skos:definition xml:lang="en">A ClassDefinition is a ComplexType which is the specification of a class, defining data attributes and methods.</skos:definition>
        <skos:example xml:lang="en">The complete source code defining the &apos;OrderProcessor&apos; class, including its fields and methods.</skos:example>
    </owl:Class>
    


    <!-- http://semantic-web-kms.edu.et/wdo#CodeBlock -->

    <owl:Class rdf:about="http://semantic-web-kms.edu.et/wdo#CodeBlock">
        <rdfs:subClassOf rdf:resource="http://semantic-web-kms.edu.et/wdo#TextualElement"/>
        <dc:identifier>WDO:0000019</dc:identifier>
        <rdfs:label xml:lang="en">Code Block</rdfs:label>
        <skos:definition xml:lang="en">A CodeBlock is a TextualElement which consists of a formatted block of example source code, typically found in READMEs or other technical documentation.</skos:definition>
        <skos:example xml:lang="en">A snippet of Python code demonstrating API usage, enclosed in triple backticks in a Markdown file.</skos:example>
    </owl:Class>
    


    <!-- http://semantic-web-kms.edu.et/wdo#CodeComment -->

    <owl:Class rdf:about="http://semantic-web-kms.edu.et/wdo#CodeComment">
        <rdfs:subClassOf rdf:resource="http://semantic-web-kms.edu.et/wdo#Documentation"/>
        <dc:identifier>WDO:0000015</dc:identifier>
        <rdfs:label xml:lang="en">Code Comment</rdfs:label>
        <skos:definition xml:lang="en">A type of Documentation which is embedded within source code to explain parts of the code. A code comment is considered atomic and cannot have further document components.</skos:definition>
        <skos:example xml:lang="en">A Javadoc block above a method explaining its purpose, parameters, and return value; an inline comment like &apos;// Temporary fix for bug #123&apos;.</skos:example>
    </owl:Class>
    


    <!-- http://semantic-web-kms.edu.et/wdo#Commit -->

    <owl:Class rdf:about="http://semantic-web-kms.edu.et/wdo#Commit">
        <rdfs:subClassOf rdf:resource="http://purl.obolibrary.org/obo/BFO_0000015"/>
        <dc:identifier>WDO:0000108</dc:identifier>
        <rdfs:label xml:lang="en">Commit</rdfs:label>
        <skos:definition xml:lang="en">A process of recording a snapshot of changes to a set of files in a repository at a specific time.</skos:definition>
    </owl:Class>
    


    <!-- http://semantic-web-kms.edu.et/wdo#ComplexType -->

    <owl:Class rdf:about="http://semantic-web-kms.edu.et/wdo#ComplexType">
        <rdfs:subClassOf rdf:resource="http://semantic-web-kms.edu.et/wdo#Type"/>
        <dc:identifier>WDO:0000006</dc:identifier>
        <rdfs:label xml:lang="en">Complex Type</rdfs:label>
        <skos:definition xml:lang="en">A ComplexType is a Type which represents a user-defined or composite data type, such as a class, interface, or enumeration. It is an abstract class.</skos:definition>
        <skos:example xml:lang="en">The definition of a &apos;UserProfile&apos; class; the specification of an &apos;Iterable&apos; interface.</skos:example>
    </owl:Class>
    


    <!-- http://semantic-web-kms.edu.et/wdo#ConfigurationFile -->

    <owl:Class rdf:about="http://semantic-web-kms.edu.et/wdo#ConfigurationFile">
        <rdfs:subClassOf rdf:resource="http://semantic-web-kms.edu.et/wdo#DigitalInformationCarrier"/>
        <dc:identifier>WDO:0000035</dc:identifier>
        <rdfs:label xml:lang="en">Configuration File</rdfs:label>
        <skos:definition xml:lang="en">A ConfigurationFile is a DigitalInformationCarrier that bears a ConfigurationSetting.</skos:definition>
        <skos:example xml:lang="en">A &apos;.env&apos; file storing environment variables; a &apos;webpack.config.js&apos; file for build configurations; a &apos;settings.json&apos; file.</skos:example>
    </owl:Class>
    


    <!-- http://semantic-web-kms.edu.et/wdo#ConfigurationSetting -->

    <owl:Class rdf:about="http://semantic-web-kms.edu.et/wdo#ConfigurationSetting">
        <rdfs:subClassOf rdf:resource="http://semantic-web-kms.edu.et/wdo#InformationContentEntity"/>
        <dc:identifier>WDO:0000022</dc:identifier>
        <rdfs:label xml:lang="en">Configuration Setting</rdfs:label>
        <skos:definition xml:lang="en">A ConfigurationSetting is an InformationContentEntity which specifies parameters or settings for a software application or system.</skos:definition>
        <skos:example xml:lang="en">The content of a &apos;database_url = ...&apos; setting in a .env file; a JSON structure defining feature flags for an application; the port number specified in a server configuration.</skos:example>
    </owl:Class>
    


    <!-- http://semantic-web-kms.edu.et/wdo#ContainerImage -->

    <owl:Class rdf:about="http://semantic-web-kms.edu.et/wdo#ContainerImage">
        <rdfs:subClassOf rdf:resource="http://semantic-web-kms.edu.et/wdo#DigitalInformationCarrier"/>
        <dc:identifier>WDO:0000110</dc:identifier>
        <rdfs:label xml:lang="en">Container Image</rdfs:label>
        <skos:definition xml:lang="en">A digital information carrier that bears a specification for creating a runnable software container. It is a standalone, executable package that includes everything needed to run a piece of software.</skos:definition>
    </owl:Class>
    


    <!-- http://semantic-web-kms.edu.et/wdo#ContributionGuide -->

    <owl:Class rdf:about="http://semantic-web-kms.edu.et/wdo#ContributionGuide">
        <rdfs:subClassOf rdf:resource="http://semantic-web-kms.edu.et/wdo#Guide"/>
        <dc:identifier>WDO:0000084</dc:identifier>
        <rdfs:label xml:lang="en">Contribution Guide</rdfs:label>
        <skos:definition xml:lang="en">A type of Guide that explains how to contribute to a project.</skos:definition>
        <skos:example xml:lang="en">A CONTRIBUTING.md file outlining the process for submitting pull requests.</skos:example>
    </owl:Class>
    


    <!-- http://semantic-web-kms.edu.et/wdo#DataFormat -->

    <owl:Class rdf:about="http://semantic-web-kms.edu.et/wdo#DataFormat">
        <rdfs:subClassOf rdf:resource="http://semantic-web-kms.edu.et/wdo#InformationContentEntity"/>
        <dc:identifier>WDO:0000095</dc:identifier>
        <rdfs:label xml:lang="en">Data Format</rdfs:label>
        <skos:definition xml:lang="en">An InformationContentEntity that defines the structure and syntax for serializing data for storage or transmission.</skos:definition>
    </owl:Class>
    


    <!-- http://semantic-web-kms.edu.et/wdo#DatabaseSchema -->

    <owl:Class rdf:about="http://semantic-web-kms.edu.et/wdo#DatabaseSchema">
        <rdfs:subClassOf rdf:resource="http://semantic-web-kms.edu.et/wdo#SQLCode"/>
        <dc:identifier>WDO:0000066</dc:identifier>
        <rdfs:label xml:lang="en">Database Schema</rdfs:label>
        <skos:definition xml:lang="en">A DatabaseSchema is a specific form of SQLCode which defines the structure, tables, columns, and relationships of a database.</skos:definition>
        <skos:example xml:lang="en">The content of a .sql file containing `CREATE TABLE` statements.</skos:example>
    </owl:Class>
    


    <!-- http://semantic-web-kms.edu.et/wdo#DatabaseSchemaFile -->

    <owl:Class rdf:about="http://semantic-web-kms.edu.et/wdo#DatabaseSchemaFile">
        <rdfs:subClassOf rdf:resource="http://semantic-web-kms.edu.et/wdo#SourceCodeFile"/>
        <dc:identifier>WDO:0000046</dc:identifier>
        <rdfs:label xml:lang="en">Database Schema File</rdfs:label>
        <skos:definition xml:lang="en">A DatabaseSchemaFile is a SourceCodeFile that bears a DatabaseSchema.</skos:definition>
        <skos:example xml:lang="en">A file named `schema.sql` or `V1__initial_setup.sql` in a Flyway migration.</skos:example>
    </owl:Class>
    


    <!-- http://semantic-web-kms.edu.et/wdo#DigitalAssetDescription -->

    <owl:Class rdf:about="http://semantic-web-kms.edu.et/wdo#DigitalAssetDescription">
        <rdfs:subClassOf rdf:resource="http://semantic-web-kms.edu.et/wdo#InformationContentEntity"/>
        <dc:identifier>WDO:0000023</dc:identifier>
        <rdfs:label xml:lang="en">Digital Asset Description</rdfs:label>
        <skos:definition xml:lang="en">A DigitalAssetDescription is an InformationContentEntity that defines the characteristics, design, plan, or descriptive metadata for a digital asset used in a web development project. This is an abstract class for specific asset descriptions.</skos:definition>
        <skos:example xml:lang="en">The description for a banner image including its required dimensions and file type; the metadata describing an audio clip&apos;s purpose and usage rights.</skos:example>
    </owl:Class>
    


    <!-- http://semantic-web-kms.edu.et/wdo#DigitalInformationCarrier -->

    <owl:Class rdf:about="http://semantic-web-kms.edu.et/wdo#DigitalInformationCarrier">
        <rdfs:subClassOf rdf:resource="http://purl.obolibrary.org/obo/BFO_0000031"/>
        <dc:identifier>WDO:0000030</dc:identifier>
        <rdfs:label xml:lang="en">Digital Information Carrier</rdfs:label>
        <skos:definition xml:lang="en">A DigitalInformationCarrier is a bfo:generically dependent continuant which is a digital object, typically a file, which encodes or bears some InformationContentEntity. This is an abstract class.</skos:definition>
        <skos:example xml:lang="en">A specific file named &apos;styles.css&apos;; an image file &apos;logo.png&apos;; a document &apos;API_Guide.pdf&apos;.</skos:example>
    </owl:Class>
    


    <!-- http://semantic-web-kms.edu.et/wdo#Dockerfile -->

    <owl:Class rdf:about="http://semantic-web-kms.edu.et/wdo#Dockerfile">
        <rdfs:subClassOf rdf:resource="http://semantic-web-kms.edu.et/wdo#DigitalInformationCarrier"/>
        <dc:identifier>WDO:0000048</dc:identifier>
        <rdfs:label xml:lang="en">Dockerfile</rdfs:label>
        <skos:definition xml:lang="en">A Dockerfile is a DigitalInformationCarrier that bears a DockerfileSpecification.</skos:definition>
        <skos:example xml:lang="en">A file named &apos;Dockerfile&apos; used to build a container image.</skos:example>
    </owl:Class>
    


    <!-- http://semantic-web-kms.edu.et/wdo#DockerfileSpecification -->

    <owl:Class rdf:about="http://semantic-web-kms.edu.et/wdo#DockerfileSpecification">
        <rdfs:subClassOf rdf:resource="http://semantic-web-kms.edu.et/wdo#InformationContentEntity"/>
        <dc:identifier>WDO:0000069</dc:identifier>
        <rdfs:label xml:lang="en">Dockerfile Specification</rdfs:label>
        <skos:definition xml:lang="en">A DockerfileSpecification is an InformationContentEntity which specifies the set of instructions for building a Docker container image.</skos:definition>
        <skos:example xml:lang="en">The sequence of commands like `FROM`, `RUN`, `COPY` inside a Dockerfile.</skos:example>
    </owl:Class>
    


    <!-- http://semantic-web-kms.edu.et/wdo#DocumentSection -->

    <owl:Class rdf:about="http://semantic-web-kms.edu.et/wdo#DocumentSection">
        <rdfs:subClassOf rdf:resource="http://semantic-web-kms.edu.et/wdo#TextualElement"/>
        <dc:identifier>WDO:0000017</dc:identifier>
        <rdfs:label xml:lang="en">Document Section</rdfs:label>
        <skos:definition xml:lang="en">A DocumentSection is a structural TextualElement whose role is to group a set of thematically related TextualElements (such as Paragraphs, Lists, and other DocumentSections) within a larger document.</skos:definition>
        <skos:example xml:lang="en">The &apos;API Endpoints&apos; section in a technical specification document; the &apos;User Stories&apos; chapter in a requirements document.</skos:example>
    </owl:Class>
    


    <!-- http://semantic-web-kms.edu.et/wdo#Documentation -->

    <owl:Class rdf:about="http://semantic-web-kms.edu.et/wdo#Documentation">
        <rdfs:subClassOf rdf:resource="http://semantic-web-kms.edu.et/wdo#InformationContentEntity"/>
        <dc:identifier>WDO:0000013</dc:identifier>
        <rdfs:label xml:lang="en">Documentation</rdfs:label>
        <skos:definition xml:lang="en">Documentation is an InformationContentEntity that provides explanatory information about a system, software, or process. It is typically composed of various document components like sections, paragraphs, and code blocks. This is an abstract class for more specific documentation types.</skos:definition>
        <skos:example xml:lang="en">The content of a user manual; API documentation generated by Javadoc; inline code comments explaining a complex algorithm.</skos:example>
    </owl:Class>
    


    <!-- http://semantic-web-kms.edu.et/wdo#DocumentationFile -->

    <owl:Class rdf:about="http://semantic-web-kms.edu.et/wdo#DocumentationFile">
        <rdfs:subClassOf rdf:resource="http://semantic-web-kms.edu.et/wdo#DigitalInformationCarrier"/>
        <dc:identifier>WDO:0000032</dc:identifier>
        <rdfs:label xml:lang="en">Documentation File</rdfs:label>
        <skos:definition xml:lang="en">A DocumentationFile is a DigitalInformationCarrier that primarily bears Documentation.</skos:definition>
        <skos:example xml:lang="en">A &apos;CONTRIBUTING.md&apos; Markdown file; a &apos;user_guide.docx&apos; Word document.</skos:example>
    </owl:Class>
    


    <!-- http://semantic-web-kms.edu.et/wdo#EnumDefinition -->

    <owl:Class rdf:about="http://semantic-web-kms.edu.et/wdo#EnumDefinition">
        <rdfs:subClassOf rdf:resource="http://semantic-web-kms.edu.et/wdo#ComplexType"/>
        <dc:identifier>WDO:0000060</dc:identifier>
        <rdfs:label xml:lang="en">Enum Definition</rdfs:label>
        <skos:definition xml:lang="en">An EnumDefinition is a ComplexType which defines an enumeration, a special data type that consists of a set of named constants.</skos:definition>
        <skos:example xml:lang="en">The definition `enum Status { PENDING, PROCESSING, COMPLETED }` in Java or TypeScript.</skos:example>
    </owl:Class>
    


    <!-- http://semantic-web-kms.edu.et/wdo#FontDescription -->

    <owl:Class rdf:about="http://semantic-web-kms.edu.et/wdo#FontDescription">
        <rdfs:subClassOf rdf:resource="http://semantic-web-kms.edu.et/wdo#DigitalAssetDescription"/>
        <dc:identifier>WDO:0000027</dc:identifier>
        <rdfs:label xml:lang="en">Font Description</rdfs:label>
        <skos:definition xml:lang="en">A FontDescription is a DigitalAssetDescription which defines the characteristics of a font, such as its family name and style.</skos:definition>
        <skos:example xml:lang="en">The description for the &apos;Open Sans&apos; font, regular weight, to be used for body text.</skos:example>
    </owl:Class>
    


    <!-- http://semantic-web-kms.edu.et/wdo#FontFile -->

    <owl:Class rdf:about="http://semantic-web-kms.edu.et/wdo#FontFile">
        <rdfs:subClassOf rdf:resource="http://semantic-web-kms.edu.et/wdo#AssetFile"/>
        <dc:identifier>WDO:0000040</dc:identifier>
        <rdfs:label xml:lang="en">Font File</rdfs:label>
        <skos:definition xml:lang="en">A FontFile is an AssetFile that bears a FontDescription.</skos:definition>
        <skos:example xml:lang="en">A file named &apos;MyCustomFont.otf&apos; or &apos;webfont.woff2&apos;.</skos:example>
    </owl:Class>
    


    <!-- http://semantic-web-kms.edu.et/wdo#FunctionCallSite -->

    <owl:Class rdf:about="http://semantic-web-kms.edu.et/wdo#FunctionCallSite">
        <rdfs:subClassOf rdf:resource="http://semantic-web-kms.edu.et/wdo#SoftwareCode"/>
        <dc:identifier>WDO:0000111</dc:identifier>
        <rdfs:label xml:lang="en">Function Call Site</rdfs:label>
        <skos:definition xml:lang="en">A FunctionCallSite is a SoftwareCode entity that represents a single, specific invocation of a function or method, including the function being called and the arguments provided.</skos:definition>
        <skos:example xml:lang="en">The specific code `calculatePrice(item, 10)` in a line of a script, which calls the &apos;calculatePrice&apos; function.</skos:example>
    </owl:Class>
    


    <!-- http://semantic-web-kms.edu.et/wdo#FunctionDefinition -->

    <owl:Class rdf:about="http://semantic-web-kms.edu.et/wdo#FunctionDefinition">
        <rdfs:subClassOf rdf:resource="http://semantic-web-kms.edu.et/wdo#SoftwareCode"/>
        <dc:identifier>WDO:0000009</dc:identifier>
        <rdfs:label xml:lang="en">Function Definition</rdfs:label>
        <skos:definition xml:lang="en">A FunctionDefinition is a SoftwareCode entity which is the specification of a function, method, or constructor.</skos:definition>
        <skos:example xml:lang="en">The source code for a &apos;getUserById(userId)&apos; method; the definition of a &apos;Product()&apos; constructor.</skos:example>
    </owl:Class>
    


    <!-- http://semantic-web-kms.edu.et/wdo#GoCode -->

    <owl:Class rdf:about="http://semantic-web-kms.edu.et/wdo#GoCode">
        <rdfs:subClassOf rdf:resource="http://semantic-web-kms.edu.et/wdo#StaticallyTypedLanguageCode"/>
        <dc:identifier>WDO:0000088</dc:identifier>
        <rdfs:label xml:lang="en">Go Code</rdfs:label>
        <skos:definition xml:lang="en">Software code written in the Go programming language.</skos:definition>
    </owl:Class>
    


    <!-- http://semantic-web-kms.edu.et/wdo#GraphQLCode -->

    <owl:Class rdf:about="http://semantic-web-kms.edu.et/wdo#GraphQLCode">
        <rdfs:subClassOf rdf:resource="http://semantic-web-kms.edu.et/wdo#QueryLanguageCode"/>
        <dc:identifier>WDO:0000090</dc:identifier>
        <rdfs:label xml:lang="en">GraphQL Code</rdfs:label>
        <skos:definition xml:lang="en">A query or schema written in the GraphQL language.</skos:definition>
    </owl:Class>
    


    <!-- http://semantic-web-kms.edu.et/wdo#Guide -->

    <owl:Class rdf:about="http://semantic-web-kms.edu.et/wdo#Guide">
        <rdfs:subClassOf rdf:resource="http://semantic-web-kms.edu.et/wdo#Documentation"/>
        <dc:identifier>WDO:0000085</dc:identifier>
        <rdfs:label xml:lang="en">Guide</rdfs:label>
        <skos:definition xml:lang="en">A type of Documentation that provides instructions or guidance on how to use, set up, or contribute to a project. This is an abstract class.</skos:definition>
    </owl:Class>
    


    <!-- http://semantic-web-kms.edu.et/wdo#HTMLCode -->

    <owl:Class rdf:about="http://semantic-web-kms.edu.et/wdo#HTMLCode">
        <rdfs:subClassOf rdf:resource="http://semantic-web-kms.edu.et/wdo#Markup"/>
        <dc:identifier>WDO:0000078</dc:identifier>
        <rdfs:label xml:lang="en">HTML Code</rdfs:label>
        <skos:definition xml:lang="en">Software code written in the HyperText Markup Language (HTML).</skos:definition>
    </owl:Class>
    


    <!-- http://semantic-web-kms.edu.et/wdo#Heading -->

    <owl:Class rdf:about="http://semantic-web-kms.edu.et/wdo#Heading">
        <rdfs:subClassOf rdf:resource="http://semantic-web-kms.edu.et/wdo#TextualElement"/>
        <dc:identifier>WDO:0000055</dc:identifier>
        <rdfs:label xml:lang="en">Heading</rdfs:label>
        <skos:definition xml:lang="en">A Heading is a TextualElement which is the title or heading that introduces a section of a document.</skos:definition>
        <skos:example xml:lang="en">The content of a markdown heading `## Installation`, which has a heading level of 2.</skos:example>
    </owl:Class>
    


    <!-- http://semantic-web-kms.edu.et/wdo#ImageDescription -->

    <owl:Class rdf:about="http://semantic-web-kms.edu.et/wdo#ImageDescription">
        <rdfs:subClassOf rdf:resource="http://semantic-web-kms.edu.et/wdo#DigitalAssetDescription"/>
        <dc:identifier>WDO:0000024</dc:identifier>
        <rdfs:label xml:lang="en">Image Description</rdfs:label>
        <skos:definition xml:lang="en">An ImageDescription is a DigitalAssetDescription which defines the characteristics of a raster or vector image, such as its dimensions, format, and color depth.</skos:definition>
        <skos:example xml:lang="en">A description for a logo image requiring SVG format, transparent background, and a maximum size of 50KB.</skos:example>
    </owl:Class>
    


    <!-- http://semantic-web-kms.edu.et/wdo#ImageFile -->

    <owl:Class rdf:about="http://semantic-web-kms.edu.et/wdo#ImageFile">
        <rdfs:subClassOf rdf:resource="http://semantic-web-kms.edu.et/wdo#AssetFile"/>
        <dc:identifier>WDO:0000037</dc:identifier>
        <rdfs:label xml:lang="en">Image File</rdfs:label>
        <skos:definition xml:lang="en">An ImageFile is an AssetFile that bears an ImageDescription.</skos:definition>
        <skos:example xml:lang="en">A file named &apos;icon.svg&apos; or &apos;background.png&apos;.</skos:example>
    </owl:Class>
    


    <!-- http://semantic-web-kms.edu.et/wdo#ImportDeclaration -->

    <owl:Class rdf:about="http://semantic-web-kms.edu.et/wdo#ImportDeclaration">
        <rdfs:subClassOf rdf:resource="http://semantic-web-kms.edu.et/wdo#SoftwareCode"/>
        <dc:identifier>WDO:0000062</dc:identifier>
        <rdfs:label xml:lang="en">Import Declaration</rdfs:label>
        <skos:definition xml:lang="en">An ImportDeclaration is a SoftwareCode entity which is a statement that makes entities from another module or package available for use in the current scope.</skos:definition>
        <skos:example xml:lang="en">The statement `import React from &apos;react&apos;;` in JavaScript or `from collections import Counter` in Python.</skos:example>
    </owl:Class>
    


    <!-- http://semantic-web-kms.edu.et/wdo#InformationContentEntity -->

    <owl:Class rdf:about="http://semantic-web-kms.edu.et/wdo#InformationContentEntity">
        <rdfs:subClassOf rdf:resource="http://purl.obolibrary.org/obo/BFO_0000031"/>
        <dc:identifier>WDO:0000002</dc:identifier>
        <rdfs:label xml:lang="en">Information Content Entity</rdfs:label>
        <skos:definition xml:lang="en">An InformationContentEntity is a bfo:generically dependent continuant that is dependent on some information bearer for its concretization and is about something. This is an abstract class.</skos:definition>
        <skos:example xml:lang="en">The textual content of a specific license agreement; the set of instructions defining a particular JavaScript function; the design description for a company logo.</skos:example>
    </owl:Class>
    


    <!-- http://semantic-web-kms.edu.et/wdo#InterfaceDefinition -->

    <owl:Class rdf:about="http://semantic-web-kms.edu.et/wdo#InterfaceDefinition">
        <rdfs:subClassOf rdf:resource="http://semantic-web-kms.edu.et/wdo#ComplexType"/>
        <dc:identifier>WDO:0000008</dc:identifier>
        <rdfs:label xml:lang="en">Interface Definition</rdfs:label>
        <skos:definition xml:lang="en">An InterfaceDefinition is a ComplexType which is the specification of an interface, defining a contract of methods.</skos:definition>
        <skos:example xml:lang="en">The content defining the &apos;Serializable&apos; interface in Java, specifying the methods that implementing classes must provide.</skos:example>
    </owl:Class>
    


    <!-- http://semantic-web-kms.edu.et/wdo#InterpretedLanguageCode -->

    <owl:Class rdf:about="http://semantic-web-kms.edu.et/wdo#InterpretedLanguageCode">
        <rdfs:subClassOf rdf:resource="http://semantic-web-kms.edu.et/wdo#SoftwareCode"/>
        <owl:disjointWith rdf:resource="http://semantic-web-kms.edu.et/wdo#StaticallyTypedLanguageCode"/>
        <dc:identifier>WDO:0000072</dc:identifier>
        <rdfs:label xml:lang="en">Interpreted Language Code</rdfs:label>
        <skos:definition xml:lang="en">Software code written in a language that is typically executed directly by an interpreter, without being compiled to machine code first. This is an abstract class.</skos:definition>
    </owl:Class>
    


    <!-- http://semantic-web-kms.edu.et/wdo#Issue -->

    <owl:Class rdf:about="http://semantic-web-kms.edu.et/wdo#Issue">
        <rdfs:subClassOf rdf:resource="http://semantic-web-kms.edu.et/wdo#InformationContentEntity"/>
        <dc:identifier>WDO:0000109</dc:identifier>
        <rdfs:label xml:lang="en">Issue</rdfs:label>
        <skos:definition xml:lang="en">An information content entity that describes a unit of work to be done, such as a bug, task, or enhancement request in a project.</skos:definition>
    </owl:Class>
    


    <!-- http://semantic-web-kms.edu.et/wdo#JSON -->

    <owl:Class rdf:about="http://semantic-web-kms.edu.et/wdo#JSON">
        <rdfs:subClassOf rdf:resource="http://semantic-web-kms.edu.et/wdo#DataFormat"/>
        <dc:identifier>WDO:0000096</dc:identifier>
        <rdfs:label xml:lang="en">JSON</rdfs:label>
        <skos:definition xml:lang="en">Data serialized in the JavaScript Object Notation (JSON) format.</skos:definition>
    </owl:Class>
    


    <!-- http://semantic-web-kms.edu.et/wdo#JavaCode -->

    <owl:Class rdf:about="http://semantic-web-kms.edu.et/wdo#JavaCode">
        <rdfs:subClassOf rdf:resource="http://semantic-web-kms.edu.et/wdo#StaticallyTypedLanguageCode"/>
        <dc:identifier>WDO:0000100</dc:identifier>
        <rdfs:label xml:lang="en">Java Code</rdfs:label>
        <skos:definition xml:lang="en">Software code written in the Java programming language.</skos:definition>
    </owl:Class>
    


    <!-- http://semantic-web-kms.edu.et/wdo#JavaScriptCode -->

    <owl:Class rdf:about="http://semantic-web-kms.edu.et/wdo#JavaScriptCode">
        <rdfs:subClassOf rdf:resource="http://semantic-web-kms.edu.et/wdo#InterpretedLanguageCode"/>
        <dc:identifier>WDO:0000074</dc:identifier>
        <rdfs:label xml:lang="en">JavaScript Code</rdfs:label>
        <skos:definition xml:lang="en">Software code written in the JavaScript programming language.</skos:definition>
    </owl:Class>
    


    <!-- http://semantic-web-kms.edu.et/wdo#JavaScriptFramework -->

    <owl:Class rdf:about="http://semantic-web-kms.edu.et/wdo#JavaScriptFramework">
        <rdfs:subClassOf rdf:resource="http://semantic-web-kms.edu.et/wdo#SoftwareFramework"/>
        <dc:identifier>WDO:0000094</dc:identifier>
        <rdfs:label xml:lang="en">JavaScript Framework</rdfs:label>
        <skos:definition xml:lang="en">A software framework written in JavaScript that provides structure for building web applications.</skos:definition>
        <skos:example xml:lang="en">React, Angular, Vue.js.</skos:example>
    </owl:Class>
    


    <!-- http://semantic-web-kms.edu.et/wdo#JupyterNotebook -->

    <owl:Class rdf:about="http://semantic-web-kms.edu.et/wdo#JupyterNotebook">
        <rdfs:subClassOf rdf:resource="http://semantic-web-kms.edu.et/wdo#Notebook"/>
        <dc:identifier>WDO:0000068</dc:identifier>
        <rdfs:label xml:lang="en">Jupyter Notebook</rdfs:label>
        <skos:definition xml:lang="en">A type of Notebook that conforms to the .ipynb format structure, commonly associated with the Jupyter project.</skos:definition>
        <skos:example xml:lang="en">The JSON content of an .ipynb file describing a sequence of executable code and documentation cells for data analysis or machine learning.</skos:example>
    </owl:Class>
    


    <!-- http://semantic-web-kms.edu.et/wdo#License -->

    <owl:Class rdf:about="http://semantic-web-kms.edu.et/wdo#License">
        <rdfs:subClassOf rdf:resource="http://semantic-web-kms.edu.et/wdo#InformationContentEntity"/>
        <dc:identifier>WDO:0000020</dc:identifier>
        <rdfs:label xml:lang="en">License</rdfs:label>
        <skos:definition xml:lang="en">A License is an InformationContentEntity that specifies the terms and conditions for software use and distribution.</skos:definition>
        <skos:example xml:lang="en">The full text of the MIT License; the specific clauses and conditions of the Apache License 2.0.</skos:example>
    </owl:Class>
    


    <!-- http://semantic-web-kms.edu.et/wdo#LicenseFile -->

    <owl:Class rdf:about="http://semantic-web-kms.edu.et/wdo#LicenseFile">
        <rdfs:subClassOf rdf:resource="http://semantic-web-kms.edu.et/wdo#DigitalInformationCarrier"/>
        <dc:identifier>WDO:0000033</dc:identifier>
        <rdfs:label xml:lang="en">License File</rdfs:label>
        <skos:definition xml:lang="en">A LicenseFile is a DigitalInformationCarrier that primarily bears a License.</skos:definition>
        <skos:example xml:lang="en">A file named &apos;LICENSE.txt&apos; containing the MIT license text.</skos:example>
    </owl:Class>
    


    <!-- http://semantic-web-kms.edu.et/wdo#List -->

    <owl:Class rdf:about="http://semantic-web-kms.edu.et/wdo#List">
        <rdfs:subClassOf rdf:resource="http://semantic-web-kms.edu.et/wdo#TextualElement"/>
        <dc:identifier>WDO:0000056</dc:identifier>
        <rdfs:label xml:lang="en">List</rdfs:label>
        <skos:definition xml:lang="en">A List is a TextualElement which consists of a series of items, typically arranged in an ordered or unordered sequence.</skos:definition>
        <skos:example xml:lang="en">An unordered list of features in a README file; an ordered list of installation steps.</skos:example>
    </owl:Class>
    


    <!-- http://semantic-web-kms.edu.et/wdo#Log -->

    <owl:Class rdf:about="http://semantic-web-kms.edu.et/wdo#Log">
        <rdfs:subClassOf rdf:resource="http://semantic-web-kms.edu.et/wdo#InformationContentEntity"/>
        <dc:identifier>WDO:0000071</dc:identifier>
        <rdfs:label xml:lang="en">Log</rdfs:label>
        <skos:definition xml:lang="en">A Log is an InformationContentEntity which is a record of events that occurred while a software application was running.</skos:definition>
        <skos:example xml:lang="en">The textual content of an application log, containing timestamped entries for errors, warnings, and informational messages.</skos:example>
    </owl:Class>
    


    <!-- http://semantic-web-kms.edu.et/wdo#LogFile -->

    <owl:Class rdf:about="http://semantic-web-kms.edu.et/wdo#LogFile">
        <rdfs:subClassOf rdf:resource="http://semantic-web-kms.edu.et/wdo#DigitalInformationCarrier"/>
        <dc:identifier>WDO:0000050</dc:identifier>
        <rdfs:label xml:lang="en">Log File</rdfs:label>
        <skos:definition xml:lang="en">A LogFile is a DigitalInformationCarrier that bears Log information.</skos:definition>
        <skos:example xml:lang="en">A file named `application.log` or `access.log`.</skos:example>
    </owl:Class>
    


    <!-- http://semantic-web-kms.edu.et/wdo#Markup -->

    <owl:Class rdf:about="http://semantic-web-kms.edu.et/wdo#Markup">
        <rdfs:subClassOf rdf:resource="http://semantic-web-kms.edu.et/wdo#InformationContentEntity"/>
        <dc:identifier>WDO:0000063</dc:identifier>
        <rdfs:label xml:lang="en">Markup</rdfs:label>
        <skos:definition xml:lang="en">Markup is an InformationContentEntity which defines the structure and presentation of a document using a system of tags.</skos:definition>
        <skos:example xml:lang="en">An HTML document defining headings, paragraphs, and links; a JSX file in a React component.</skos:example>
    </owl:Class>
    


    <!-- http://semantic-web-kms.edu.et/wdo#MarkupFile -->

    <owl:Class rdf:about="http://semantic-web-kms.edu.et/wdo#MarkupFile">
        <rdfs:subClassOf rdf:resource="http://semantic-web-kms.edu.et/wdo#DigitalInformationCarrier"/>
        <dc:identifier>WDO:0000043</dc:identifier>
        <rdfs:label xml:lang="en">Markup File</rdfs:label>
        <skos:definition xml:lang="en">A MarkupFile is a DigitalInformationCarrier that bears Markup.</skos:definition>
        <skos:example xml:lang="en">A file named `index.html`, `main.jsx`, or `document.xml`.</skos:example>
    </owl:Class>
    


    <!-- http://semantic-web-kms.edu.et/wdo#Module -->

    <owl:Class rdf:about="http://semantic-web-kms.edu.et/wdo#Module">
        <rdfs:subClassOf rdf:resource="http://semantic-web-kms.edu.et/wdo#SoftwarePackage"/>
        <dc:identifier>WDO:0000061</dc:identifier>
        <rdfs:comment xml:lang="en">Design Note: A module is modeled as a specific kind of package, typically one corresponding to a single file. In some language ecosystems, the relationship might be better modeled as `part-of`, but `is-a` is used here as a practical simplification.</rdfs:comment>
        <rdfs:label xml:lang="en">Module</rdfs:label>
        <skos:definition xml:lang="en">A Module is a SoftwarePackage which is the specification of a single, self-contained unit of code (often a single file) that can be imported and reused.</skos:definition>
        <skos:example xml:lang="en">A Python file (`utils.py`) or a JavaScript file (`api.js`) that exports functions or classes.</skos:example>
    </owl:Class>
    


    <!-- http://semantic-web-kms.edu.et/wdo#ModuleFile -->

    <owl:Class rdf:about="http://semantic-web-kms.edu.et/wdo#ModuleFile">
        <rdfs:subClassOf rdf:resource="http://semantic-web-kms.edu.et/wdo#SourceCodeFile"/>
        <dc:identifier>WDO:0000105</dc:identifier>
        <rdfs:label xml:lang="en">Module File</rdfs:label>
        <skos:definition xml:lang="en">A type of SourceCodeFile whose primary role is to define reusable logic or components intended to be imported by other parts of an application.</skos:definition>
        <skos:example xml:lang="en">A file named `UserService.js` defining a class to be used elsewhere; `database.py` containing connection logic; a React component file like `Button.tsx`.</skos:example>
    </owl:Class>
    


    <!-- http://semantic-web-kms.edu.et/wdo#Notebook -->

    <owl:Class rdf:about="http://semantic-web-kms.edu.et/wdo#Notebook">
        <rdfs:subClassOf rdf:resource="http://semantic-web-kms.edu.et/wdo#InformationContentEntity"/>
        <dc:identifier>WDO:0000104</dc:identifier>
        <rdfs:label xml:lang="en">Notebook</rdfs:label>
        <skos:definition xml:lang="en">An InformationContentEntity which represents the structured content of a computational notebook, including code cells, markdown cells, and outputs.</skos:definition>
    </owl:Class>
    


    <!-- http://semantic-web-kms.edu.et/wdo#NotebookFile -->

    <owl:Class rdf:about="http://semantic-web-kms.edu.et/wdo#NotebookFile">
        <rdfs:subClassOf rdf:resource="http://semantic-web-kms.edu.et/wdo#DigitalInformationCarrier"/>
        <dc:identifier>WDO:0000047</dc:identifier>
        <rdfs:label xml:lang="en">Notebook File</rdfs:label>
        <skos:definition xml:lang="en">A NotebookFile is a DigitalInformationCarrier that bears Notebook content.</skos:definition>
        <skos:example xml:lang="en">A file named `data_analysis.ipynb`.</skos:example>
    </owl:Class>
    


    <!-- http://semantic-web-kms.edu.et/wdo#Organization -->

    <owl:Class rdf:about="http://semantic-web-kms.edu.et/wdo#Organization">
        <rdfs:subClassOf rdf:resource="http://purl.obolibrary.org/obo/BFO_0000040"/>
        <rdfs:comment xml:lang="en">An organization is a material entity in BFO, and serves as the top-level entity for repositories and assets.</rdfs:comment>
        <skos:definition xml:lang="en">A social or legal entity such as a company, institution, or group, which acts as an agent and can own assets, employ people, and manage projects. In this ontology, an organization is the root entity for its repositories and digital assets.</skos:definition>
        <skos:example xml:lang="en">A software company like &apos;Thinkster&apos;, a university department, or an open-source foundation. For example, &apos;Thinkster&apos; is a wdo:Organization that owns several repositories.</skos:example>
    </owl:Class>
    


    <!-- http://semantic-web-kms.edu.et/wdo#PHPCode -->

    <owl:Class rdf:about="http://semantic-web-kms.edu.et/wdo#PHPCode">
        <rdfs:subClassOf rdf:resource="http://semantic-web-kms.edu.et/wdo#InterpretedLanguageCode"/>
        <dc:identifier>WDO:0000086</dc:identifier>
        <rdfs:label xml:lang="en">PHP Code</rdfs:label>
        <skos:definition xml:lang="en">Software code written in the PHP programming language.</skos:definition>
    </owl:Class>
    


    <!-- http://semantic-web-kms.edu.et/wdo#Paragraph -->

    <owl:Class rdf:about="http://semantic-web-kms.edu.et/wdo#Paragraph">
        <rdfs:subClassOf rdf:resource="http://semantic-web-kms.edu.et/wdo#TextualElement"/>
        <dc:identifier>WDO:0000018</dc:identifier>
        <rdfs:label xml:lang="en">Paragraph</rdfs:label>
        <skos:definition xml:lang="en">A Paragraph is a TextualElement which is a self-contained unit of discourse dealing with a particular point or idea, typically composed of one or more sentences.</skos:definition>
        <skos:example xml:lang="en">A block of text in a README file explaining a specific feature.</skos:example>
    </owl:Class>
    


    <!-- http://semantic-web-kms.edu.et/wdo#Parameter -->

    <owl:Class rdf:about="http://semantic-web-kms.edu.et/wdo#Parameter">
        <rdfs:subClassOf rdf:resource="http://semantic-web-kms.edu.et/wdo#SoftwareCode"/>
        <dc:identifier>WDO:0000011</dc:identifier>
        <rdfs:label xml:lang="en">Parameter</rdfs:label>
        <skos:definition xml:lang="en">A Parameter is a SoftwareCode entity which is the specification of a parameter for a function or method.</skos:definition>
        <skos:example xml:lang="en">The &apos;int count&apos; parameter in a function signature &apos;void printItems(int count)&apos;; the &apos;options: object&apos; parameter in a TypeScript function.</skos:example>
    </owl:Class>
    


    <!-- http://semantic-web-kms.edu.et/wdo#PrimitiveType -->

    <owl:Class rdf:about="http://semantic-web-kms.edu.et/wdo#PrimitiveType">
        <rdfs:subClassOf rdf:resource="http://semantic-web-kms.edu.et/wdo#Type"/>
        <dc:identifier>WDO:0000005</dc:identifier>
        <rdfs:label xml:lang="en">Primitive Type</rdfs:label>
        <skos:definition xml:lang="en">A PrimitiveType is a Type which represents a basic data type provided by a programming language, such as integer, boolean, or character.</skos:definition>
        <skos:example xml:lang="en">The &apos;boolean&apos; type in Python; the &apos;int&apos; type specification in C++.</skos:example>
    </owl:Class>
    


    <!-- http://semantic-web-kms.edu.et/wdo#PythonCode -->

    <owl:Class rdf:about="http://semantic-web-kms.edu.et/wdo#PythonCode">
        <rdfs:subClassOf rdf:resource="http://semantic-web-kms.edu.et/wdo#InterpretedLanguageCode"/>
        <dc:identifier>WDO:0000073</dc:identifier>
        <rdfs:label xml:lang="en">Python Code</rdfs:label>
        <skos:definition xml:lang="en">Software code written in the Python programming language.</skos:definition>
    </owl:Class>
    


    <!-- http://semantic-web-kms.edu.et/wdo#QueryLanguageCode -->

    <owl:Class rdf:about="http://semantic-web-kms.edu.et/wdo#QueryLanguageCode">
        <rdfs:subClassOf rdf:resource="http://semantic-web-kms.edu.et/wdo#SoftwareCode"/>
        <dc:identifier>WDO:0000091</dc:identifier>
        <rdfs:label xml:lang="en">Query Language Code</rdfs:label>
        <skos:definition xml:lang="en">Software code written in a language used to make queries in databases and information systems. This is an abstract class.</skos:definition>
    </owl:Class>
    


    <!-- http://semantic-web-kms.edu.et/wdo#Readme -->

    <owl:Class rdf:about="http://semantic-web-kms.edu.et/wdo#Readme">
        <rdfs:subClassOf rdf:resource="http://semantic-web-kms.edu.et/wdo#Documentation"/>
        <dc:identifier>WDO:0000014</dc:identifier>
        <rdfs:label xml:lang="en">Readme</rdfs:label>
        <skos:definition xml:lang="en">A Readme is a type of Documentation that provides essential information about a software project.</skos:definition>
        <skos:example xml:lang="en">The textual content and structure within a &apos;README.md&apos; file, including sections like &apos;Installation&apos;, &apos;Usage&apos;, and &apos;Contributing&apos;.</skos:example>
    </owl:Class>
    


    <!-- http://semantic-web-kms.edu.et/wdo#ReadmeFile -->

    <owl:Class rdf:about="http://semantic-web-kms.edu.et/wdo#ReadmeFile">
        <rdfs:subClassOf rdf:resource="http://semantic-web-kms.edu.et/wdo#DocumentationFile"/>
        <dc:identifier>WDO:0000034</dc:identifier>
        <rdfs:label xml:lang="en">Readme File</rdfs:label>
        <skos:definition xml:lang="en">A ReadmeFile is a DocumentationFile that bears Readme information.</skos:definition>
        <skos:example xml:lang="en">The &apos;README.md&apos; file at the root of a GitHub repository.</skos:example>
    </owl:Class>
    


    <!-- http://semantic-web-kms.edu.et/wdo#Repository -->

    <owl:Class rdf:about="http://semantic-web-kms.edu.et/wdo#Repository">
        <rdfs:subClassOf rdf:resource="http://purl.obolibrary.org/obo/BFO_0000040"/>
        <dc:identifier>WDO:0000107</dc:identifier>
        <rdfs:label xml:lang="en">Repository</rdfs:label>
        <skos:definition xml:lang="en">An object aggregate consisting of a collection of digital information carriers (files) and their revision history.</skos:definition>
    </owl:Class>
    


    <!-- http://semantic-web-kms.edu.et/wdo#RubyCode -->

    <owl:Class rdf:about="http://semantic-web-kms.edu.et/wdo#RubyCode">
        <rdfs:subClassOf rdf:resource="http://semantic-web-kms.edu.et/wdo#InterpretedLanguageCode"/>
        <dc:identifier>WDO:0000087</dc:identifier>
        <rdfs:label xml:lang="en">Ruby Code</rdfs:label>
        <skos:definition xml:lang="en">Software code written in the Ruby programming language.</skos:definition>
    </owl:Class>
    


    <!-- http://semantic-web-kms.edu.et/wdo#RustCode -->

    <owl:Class rdf:about="http://semantic-web-kms.edu.et/wdo#RustCode">
        <rdfs:subClassOf rdf:resource="http://semantic-web-kms.edu.et/wdo#StaticallyTypedLanguageCode"/>
        <dc:identifier>WDO:0000102</dc:identifier>
        <rdfs:label xml:lang="en">Rust Code</rdfs:label>
        <skos:definition xml:lang="en">Software code written in the Rust programming language, known for its performance and safety features.</skos:definition>
    </owl:Class>
    


    <!-- http://semantic-web-kms.edu.et/wdo#SQLCode -->

    <owl:Class rdf:about="http://semantic-web-kms.edu.et/wdo#SQLCode">
        <rdfs:subClassOf rdf:resource="http://semantic-web-kms.edu.et/wdo#QueryLanguageCode"/>
        <dc:identifier>WDO:0000089</dc:identifier>
        <rdfs:label xml:lang="en">SQL Code</rdfs:label>
        <skos:definition xml:lang="en">A query or schema written in the Structured Query Language (SQL).</skos:definition>
    </owl:Class>
    


    <!-- http://semantic-web-kms.edu.et/wdo#ScriptFile -->

    <owl:Class rdf:about="http://semantic-web-kms.edu.et/wdo#ScriptFile">
        <rdfs:subClassOf rdf:resource="http://semantic-web-kms.edu.et/wdo#SourceCodeFile"/>
        <dc:identifier>WDO:0000051</dc:identifier>
        <rdfs:label xml:lang="en">Script File</rdfs:label>
        <skos:definition xml:lang="en">A ScriptFile is a SourceCodeFile that bears script code intended for direct execution to perform a specific task.</skos:definition>
        <skos:example xml:lang="en">A file named `myscript.sh`, `task.py`, or `automation.js`.</skos:example>
    </owl:Class>
    


    <!-- http://semantic-web-kms.edu.et/wdo#SoftwareCode -->

    <owl:Class rdf:about="http://semantic-web-kms.edu.et/wdo#SoftwareCode">
        <rdfs:subClassOf rdf:resource="http://semantic-web-kms.edu.et/wdo#InformationContentEntity"/>
        <dc:identifier>WDO:0000003</dc:identifier>
        <rdfs:label xml:lang="en">Software Code</rdfs:label>
        <skos:definition xml:lang="en">SoftwareCode is an InformationContentEntity which is a set of instructions or declarations written in a programming language. This is an abstract class.</skos:definition>
        <skos:example xml:lang="en">A &apos;User.java&apos; class definition; the specific algorithm encoded in a &apos;calculatePrice&apos; function; the declarations within a CSS stylesheet.</skos:example>
    </owl:Class>
    


    <!-- http://semantic-web-kms.edu.et/wdo#SoftwareFramework -->

    <owl:Class rdf:about="http://semantic-web-kms.edu.et/wdo#SoftwareFramework">
        <rdfs:subClassOf rdf:resource="http://semantic-web-kms.edu.et/wdo#InformationContentEntity"/>
        <dc:identifier>WDO:0000092</dc:identifier>
        <rdfs:label xml:lang="en">Software Framework</rdfs:label>
        <skos:definition xml:lang="en">An InformationContentEntity that provides a reusable, generic platform of code and assets for software applications, so that developers can focus on the specific logic of their application.</skos:definition>
    </owl:Class>
    


    <!-- http://semantic-web-kms.edu.et/wdo#SoftwarePackage -->

    <owl:Class rdf:about="http://semantic-web-kms.edu.et/wdo#SoftwarePackage">
        <rdfs:subClassOf rdf:resource="http://semantic-web-kms.edu.et/wdo#SoftwareCode"/>
        <dc:identifier>WDO:0000012</dc:identifier>
        <rdfs:label xml:lang="en">Software Package</rdfs:label>
        <skos:definition xml:lang="en">A SoftwarePackage is a SoftwareCode entity which represents the specification of a software package or namespace, a mechanism for organizing code elements. This is an abstract class.</skos:definition>
        <skos:example xml:lang="en">The declaration &apos;package com.example.utils;&apos; in a Java file; the conceptual grouping of modules under a &apos;services&apos; directory in a Python project.</skos:example>
    </owl:Class>
    


    <!-- http://semantic-web-kms.edu.et/wdo#SourceCodeFile -->

    <owl:Class rdf:about="http://semantic-web-kms.edu.et/wdo#SourceCodeFile">
        <rdfs:subClassOf rdf:resource="http://semantic-web-kms.edu.et/wdo#DigitalInformationCarrier"/>
        <dc:identifier>WDO:0000031</dc:identifier>
        <rdfs:label xml:lang="en">Source Code File</rdfs:label>
        <skos:definition xml:lang="en">A SourceCodeFile is a DigitalInformationCarrier that primarily bears SoftwareCode. This is an abstract class.</skos:definition>
        <skos:example xml:lang="en">The file &apos;server.js&apos; containing JavaScript code; &apos;database_schema.sql&apos; containing SQL DDL statements.</skos:example>
    </owl:Class>
    


    <!-- http://semantic-web-kms.edu.et/wdo#StaticallyTypedLanguageCode -->

    <owl:Class rdf:about="http://semantic-web-kms.edu.et/wdo#StaticallyTypedLanguageCode">
        <rdfs:subClassOf rdf:resource="http://semantic-web-kms.edu.et/wdo#SoftwareCode"/>
        <dc:identifier>WDO:0000080</dc:identifier>
        <rdfs:label xml:lang="en">Statically Typed Language Code</rdfs:label>
        <skos:definition xml:lang="en">Software code written in a language where variable types are checked at compile-time rather than at runtime. This is an abstract class.</skos:definition>
    </owl:Class>
    


    <!-- http://semantic-web-kms.edu.et/wdo#StructDefinition -->

    <owl:Class rdf:about="http://semantic-web-kms.edu.et/wdo#StructDefinition">
        <rdfs:subClassOf rdf:resource="http://semantic-web-kms.edu.et/wdo#ComplexType"/>
        <dc:identifier>WDO:0000059</dc:identifier>
        <rdfs:label xml:lang="en">Struct Definition</rdfs:label>
        <skos:definition xml:lang="en">A StructDefinition is a ComplexType which defines a struct, a composite data type that groups variables under a single name.</skos:definition>
        <skos:example xml:lang="en">The definition `struct Point { int x; int y; }` in C or Golang.</skos:example>
    </owl:Class>
    


    <!-- http://semantic-web-kms.edu.et/wdo#Stylesheet -->

    <owl:Class rdf:about="http://semantic-web-kms.edu.et/wdo#Stylesheet">
        <rdfs:subClassOf rdf:resource="http://semantic-web-kms.edu.et/wdo#SoftwareCode"/>
        <dc:identifier>WDO:0000064</dc:identifier>
        <rdfs:label xml:lang="en">Stylesheet</rdfs:label>
        <skos:definition xml:lang="en">A Stylesheet is a SoftwareCode entity which defines the presentation and styling rules for a markup document.</skos:definition>
        <skos:example xml:lang="en">A CSS file defining colors, fonts, and layout; an SASS or LESS file.</skos:example>
    </owl:Class>
    


    <!-- http://semantic-web-kms.edu.et/wdo#StylesheetFile -->

    <owl:Class rdf:about="http://semantic-web-kms.edu.et/wdo#StylesheetFile">
        <rdfs:subClassOf rdf:resource="http://semantic-web-kms.edu.et/wdo#DigitalInformationCarrier"/>
        <dc:identifier>WDO:0000044</dc:identifier>
        <rdfs:label xml:lang="en">Stylesheet File</rdfs:label>
        <skos:definition xml:lang="en">A StylesheetFile is a DigitalInformationCarrier that bears a Stylesheet.</skos:definition>
        <skos:example xml:lang="en">A file named `styles.css` or `theme.scss`.</skos:example>
    </owl:Class>
    


    <!-- http://semantic-web-kms.edu.et/wdo#Table -->

    <owl:Class rdf:about="http://semantic-web-kms.edu.et/wdo#Table">
        <rdfs:subClassOf rdf:resource="http://semantic-web-kms.edu.et/wdo#TextualElement"/>
        <dc:identifier>WDO:0000058</dc:identifier>
        <rdfs:label xml:lang="en">Table</rdfs:label>
        <skos:definition xml:lang="en">A Table is a TextualElement which consists of data arranged in rows and columns.</skos:definition>
        <skos:example xml:lang="en">A table comparing feature plans in a project&apos;s documentation, often created with pipe characters (`|`) in Markdown.</skos:example>
    </owl:Class>
    


    <!-- http://semantic-web-kms.edu.et/wdo#Template -->

    <owl:Class rdf:about="http://semantic-web-kms.edu.et/wdo#Template">
        <rdfs:subClassOf rdf:resource="http://semantic-web-kms.edu.et/wdo#Markup"/>
        <dc:identifier>WDO:0000065</dc:identifier>
        <rdfs:label xml:lang="en">Template</rdfs:label>
        <skos:definition xml:lang="en">A Template is a type of Markup which defines a pre-formatted structure that can be filled with data to produce a final document.</skos:definition>
        <skos:example xml:lang="en">A Handlebars (.hbs) or EJS (.ejs) file containing placeholders for dynamic data.</skos:example>
    </owl:Class>
    


    <!-- http://semantic-web-kms.edu.et/wdo#TemplateFile -->

    <owl:Class rdf:about="http://semantic-web-kms.edu.et/wdo#TemplateFile">
        <rdfs:subClassOf rdf:resource="http://semantic-web-kms.edu.et/wdo#MarkupFile"/>
        <dc:identifier>WDO:0000045</dc:identifier>
        <rdfs:label xml:lang="en">Template File</rdfs:label>
        <skos:definition xml:lang="en">A TemplateFile is a MarkupFile that bears a Template.</skos:definition>
        <skos:example xml:lang="en">A file named `user_profile.hbs` or `email_template.ejs`.</skos:example>
    </owl:Class>
    


    <!-- http://semantic-web-kms.edu.et/wdo#TestFile -->

    <owl:Class rdf:about="http://semantic-web-kms.edu.et/wdo#TestFile">
        <rdfs:subClassOf rdf:resource="http://semantic-web-kms.edu.et/wdo#SourceCodeFile"/>
        <dc:identifier>WDO:0000106</dc:identifier>
        <rdfs:label xml:lang="en">Test File</rdfs:label>
        <skos:definition xml:lang="en">A type of SourceCodeFile whose primary role is to bear code that verifies the correctness of other software code.</skos:definition>
        <skos:example xml:lang="en">A file named `auth.test.js` using Jest; `test_models.py` using PyTest.</skos:example>
    </owl:Class>
    


    <!-- http://semantic-web-kms.edu.et/wdo#TextualElement -->

    <owl:Class rdf:about="http://semantic-web-kms.edu.et/wdo#TextualElement">
        <rdfs:subClassOf rdf:resource="http://semantic-web-kms.edu.et/wdo#InformationContentEntity"/>
        <dc:identifier>WDO:0000016</dc:identifier>
        <rdfs:label xml:lang="en">Textual Element</rdfs:label>
        <skos:definition xml:lang="en">A TextualElement is an InformationContentEntity which is a discrete piece of text, such as a title, caption, or sentence, forming part of a larger document structure.</skos:definition>
        <skos:example xml:lang="en">The content of a heading &apos;&lt;h2&gt;Setup Instructions&lt;/h2&gt;&apos;; the text of a single sentence within a paragraph; a figure caption like &apos;Figure 1: System Architecture&apos;.</skos:example>
    </owl:Class>
    


    <!-- http://semantic-web-kms.edu.et/wdo#ThreeDimensionalModelDescription -->

    <owl:Class rdf:about="http://semantic-web-kms.edu.et/wdo#ThreeDimensionalModelDescription">
        <rdfs:subClassOf rdf:resource="http://semantic-web-kms.edu.et/wdo#DigitalAssetDescription"/>
        <dc:identifier>WDO:0000028</dc:identifier>
        <rdfs:label xml:lang="en">Three-Dimensional Model Description</rdfs:label>
        <skos:definition xml:lang="en">A ThreeDimensionalModelDescription is a DigitalAssetDescription which defines the characteristics of a 3D model, such as its geometry, textures, and format.</skos:definition>
        <skos:example xml:lang="en">The description for a 3D product model in GLTF format, including polygon count limits and texture map requirements.</skos:example>
    </owl:Class>
    


    <!-- http://semantic-web-kms.edu.et/wdo#ThreeDimensionalModelFile -->

    <owl:Class rdf:about="http://semantic-web-kms.edu.et/wdo#ThreeDimensionalModelFile">
        <rdfs:subClassOf rdf:resource="http://semantic-web-kms.edu.et/wdo#AssetFile"/>
        <dc:identifier>WDO:0000041</dc:identifier>
        <rdfs:label xml:lang="en">Three-Dimensional Model File</rdfs:label>
        <skos:definition xml:lang="en">A ThreeDimensionalModelFile is an AssetFile that bears a ThreeDimensionalModelDescription.</skos:definition>
        <skos:example xml:lang="en">A file named &apos;product_model.glb&apos; or &apos;character.fbx&apos;.</skos:example>
    </owl:Class>
    


    <!-- http://semantic-web-kms.edu.et/wdo#Tutorial -->

    <owl:Class rdf:about="http://semantic-web-kms.edu.et/wdo#Tutorial">
        <rdfs:subClassOf rdf:resource="http://semantic-web-kms.edu.et/wdo#Guide"/>
        <dc:identifier>WDO:0000099</dc:identifier>
        <rdfs:label xml:lang="en">Tutorial</rdfs:label>
        <skos:definition xml:lang="en">A type of Guide that provides step-by-step instructions to complete a specific task.</skos:definition>
    </owl:Class>
    


    <!-- http://semantic-web-kms.edu.et/wdo#Type -->

    <owl:Class rdf:about="http://semantic-web-kms.edu.et/wdo#Type">
        <rdfs:subClassOf rdf:resource="http://semantic-web-kms.edu.et/wdo#SoftwareCode"/>
        <dc:identifier>WDO:0000004</dc:identifier>
        <rdfs:label xml:lang="en">Type</rdfs:label>
        <skos:definition xml:lang="en">A Type is a SoftwareCode entity which represents the specification of a data type in a programming language. This is an abstract class.</skos:definition>
        <skos:example xml:lang="en">The specification of an &apos;integer&apos; type in Java; the definition of a &apos;String&apos; type; the structure of a &apos;CustomerRecord&apos; complex type.</skos:example>
    </owl:Class>
    


    <!-- http://semantic-web-kms.edu.et/wdo#TypeScriptCode -->

    <owl:Class rdf:about="http://semantic-web-kms.edu.et/wdo#TypeScriptCode">
        <rdfs:subClassOf rdf:resource="http://semantic-web-kms.edu.et/wdo#StaticallyTypedLanguageCode"/>
        <dc:identifier>WDO:0000075</dc:identifier>
        <rdfs:label xml:lang="en">TypeScript Code</rdfs:label>
        <skos:definition xml:lang="en">Software code written in the TypeScript programming language, a superset of JavaScript that adds static typing.</skos:definition>
    </owl:Class>
    


    <!-- http://semantic-web-kms.edu.et/wdo#UserGuide -->

    <owl:Class rdf:about="http://semantic-web-kms.edu.et/wdo#UserGuide">
        <rdfs:subClassOf rdf:resource="http://semantic-web-kms.edu.et/wdo#Guide"/>
        <dc:identifier>WDO:0000103</dc:identifier>
        <rdfs:label xml:lang="en">User Guide</rdfs:label>
        <skos:definition xml:lang="en">A type of Guide that explains how to use a software product or system from the perspective of an end-user.</skos:definition>
    </owl:Class>
    


    <!-- http://semantic-web-kms.edu.et/wdo#UserInterfaceDesignDescription -->

    <owl:Class rdf:about="http://semantic-web-kms.edu.et/wdo#UserInterfaceDesignDescription">
        <rdfs:subClassOf rdf:resource="http://semantic-web-kms.edu.et/wdo#DigitalAssetDescription"/>
        <dc:identifier>WDO:0000029</dc:identifier>
        <rdfs:label xml:lang="en">User Interface Design Description</rdfs:label>
        <skos:definition xml:lang="en">A UserInterfaceDesignDescription is a DigitalAssetDescription which defines the characteristics of a user interface design, such as wireframes, mockups, or prototypes.</skos:definition>
        <skos:example xml:lang="en">A wireframe design for a mobile application&apos;s login screen; a high-fidelity mockup of a website homepage created in Figma.</skos:example>
    </owl:Class>
    


    <!-- http://semantic-web-kms.edu.et/wdo#UserInterfaceDesignFile -->

    <owl:Class rdf:about="http://semantic-web-kms.edu.et/wdo#UserInterfaceDesignFile">
        <rdfs:subClassOf rdf:resource="http://semantic-web-kms.edu.et/wdo#AssetFile"/>
        <dc:identifier>WDO:0000042</dc:identifier>
        <rdfs:label xml:lang="en">User Interface Design File</rdfs:label>
        <skos:definition xml:lang="en">A UserInterfaceDesignFile is an AssetFile that bears a UserInterfaceDesignDescription (e.g., a Figma, Sketch, or Adobe XD file).</skos:definition>
        <skos:example xml:lang="en">A file named &apos;homepage_mockup.fig&apos; or &apos;app_prototype.xd&apos;.</skos:example>
    </owl:Class>
    


    <!-- http://semantic-web-kms.edu.et/wdo#VariableDeclaration -->

    <owl:Class rdf:about="http://semantic-web-kms.edu.et/wdo#VariableDeclaration">
        <rdfs:subClassOf rdf:resource="http://semantic-web-kms.edu.et/wdo#SoftwareCode"/>
        <dc:identifier>WDO:0000067</dc:identifier>
        <rdfs:label xml:lang="en">Variable Declaration</rdfs:label>
        <skos:definition xml:lang="en">A VariableDeclaration is a SoftwareCode entity which is the declaration of a variable within a local scope, such as a function body.</skos:definition>
        <skos:example xml:lang="en">The declaration `let counter = 0;` inside a JavaScript function.</skos:example>
    </owl:Class>
    


    <!-- http://semantic-web-kms.edu.et/wdo#VideoDescription -->

    <owl:Class rdf:about="http://semantic-web-kms.edu.et/wdo#VideoDescription">
        <rdfs:subClassOf rdf:resource="http://semantic-web-kms.edu.et/wdo#DigitalAssetDescription"/>
        <dc:identifier>WDO:0000025</dc:identifier>
        <rdfs:label xml:lang="en">Video Description</rdfs:label>
        <skos:definition xml:lang="en">A VideoDescription is a DigitalAssetDescription which defines the characteristics of a video, such as its duration, frame rate, and encoding.</skos:definition>
        <skos:example xml:lang="en">A description for a tutorial video requiring MP4 format, 1080p resolution, H.264 encoding, and a duration not exceeding 5 minutes.</skos:example>
    </owl:Class>
    


    <!-- http://semantic-web-kms.edu.et/wdo#VideoFile -->

    <owl:Class rdf:about="http://semantic-web-kms.edu.et/wdo#VideoFile">
        <rdfs:subClassOf rdf:resource="http://semantic-web-kms.edu.et/wdo#AssetFile"/>
        <dc:identifier>WDO:0000038</dc:identifier>
        <rdfs:label xml:lang="en">Video File</rdfs:label>
        <skos:definition xml:lang="en">A VideoFile is an AssetFile that bears a VideoDescription.</skos:definition>
        <skos:example xml:lang="en">A file named &apos;tutorial.mp4&apos; or &apos;promo.webm&apos;.</skos:example>
    </owl:Class>
    


    <!-- http://semantic-web-kms.edu.et/wdo#WebDevelopmentProject -->

    <owl:Class rdf:about="http://semantic-web-kms.edu.et/wdo#WebDevelopmentProject">
        <rdfs:subClassOf rdf:resource="http://purl.obolibrary.org/obo/BFO_0000015"/>
        <dc:identifier>WDO:0000001</dc:identifier>
        <rdfs:label xml:lang="en">Web Development Project</rdfs:label>
        <skos:definition xml:lang="en">A WebDevelopmentProject is a bfo:process that encompasses all activities, planning, and execution involved in creating, deploying, or maintaining a web-based software application or system.</skos:definition>
        <skos:example xml:lang="en">The &apos;Apollo E-commerce Platform Upgrade&apos; project aiming to refactor the checkout module and integrate a new payment gateway over three months.</skos:example>
    </owl:Class>
    


    <!-- http://semantic-web-kms.edu.et/wdo#XML -->

    <owl:Class rdf:about="http://semantic-web-kms.edu.et/wdo#XML">
        <rdfs:subClassOf rdf:resource="http://semantic-web-kms.edu.et/wdo#DataFormat"/>
        <dc:identifier>WDO:0000097</dc:identifier>
        <rdfs:label xml:lang="en">XML</rdfs:label>
        <skos:definition xml:lang="en">Data serialized in the Extensible Markup Language (XML) format.</skos:definition>
    </owl:Class>
    


    <!-- http://semantic-web-kms.edu.et/wdo#YAML -->

    <owl:Class rdf:about="http://semantic-web-kms.edu.et/wdo#YAML">
        <rdfs:subClassOf rdf:resource="http://semantic-web-kms.edu.et/wdo#DataFormat"/>
        <dc:identifier>WDO:0000098</dc:identifier>
        <rdfs:label xml:lang="en">YAML</rdfs:label>
        <skos:definition xml:lang="en">Data serialized in the YAML Ain&apos;t Markup Language (YAML) format.</skos:definition>
    </owl:Class>


    
    <!-- http://semantic-web-kms.edu.et/wdo#CommitMessage -->
    <owl:Class rdf:about="http://semantic-web-kms.edu.et/wdo#CommitMessage">
        <rdfs:subClassOf rdf:resource="http://semantic-web-kms.edu.et/wdo#InformationContentEntity"/>
        <rdfs:label xml:lang="en">Commit Message</rdfs:label>
        <skos:definition xml:lang="en">A textual message describing the changes made in a specific commit in a version control system.</skos:definition>
        <skos:example xml:lang="en">"Fix bug in user authentication logic"</skos:example>
    </owl:Class>


    
    <!-- http://semantic-web-kms.edu.et/wdo#hasCommitMessage -->
    <owl:ObjectProperty rdf:about="http://semantic-web-kms.edu.et/wdo#hasCommitMessage">
        <rdfs:domain rdf:resource="http://semantic-web-kms.edu.et/wdo#Commit"/>
        <rdfs:range rdf:resource="http://semantic-web-kms.edu.et/wdo#CommitMessage"/>
        <rdfs:label xml:lang="en">has commit message</rdfs:label>
        <skos:definition xml:lang="en">A relation linking a Commit process to its associated CommitMessage entity. Use this instead of bearerOfInformation for commit messages.</skos:definition>
    </owl:ObjectProperty>
    <!-- NOTE: Do NOT use bearerOfInformation between Commit and CommitMessage. -->

    <!-- http://semantic-web-kms.edu.et/wdo#hasFile -->
    <owl:ObjectProperty rdf:about="http://semantic-web-kms.edu.et/wdo#hasFile">
        <rdfs:domain rdf:resource="http://semantic-web-kms.edu.et/wdo#Repository"/>
        <rdfs:range rdf:resource="http://semantic-web-kms.edu.et/wdo#DigitalInformationCarrier"/>
        <rdfs:label xml:lang="en">has file</rdfs:label>
        <skos:definition xml:lang="en">A relation linking a repository to the digital information carriers (files) it contains.</skos:definition>
    </owl:ObjectProperty>
</rdf:RDF>



<!-- Generated by the OWL API (version 4.5.29.2024-05-13T12:11:03Z) https://github.com/owlcs/owlapi -->
